1) redefined memory model interfaces to be only a mapping from addresses to bytes, with a table to store allocated blocks. This is very close to the memory model in Softbound+CETS, but it also considers data layouts of different types (not only atomic types), providing a family of functions that interprete sequences of bytes into values of different types. In dynamic semantics, values are sequences of bytes.
2) added 'sequence of instructions to run within the current block' into
ExecutionContext, because 'getNextInsn' doesn't work when looking for the next
instruction ready to run according to the current instruction.
'getNextInsn' used 'id' of each instruction to uniquely (becasue of SSA) identify instructions, however, some instructions, such as 'store', don't have such ids.

3) moved trace definitions into 'trace.v'



git-svn-id: https://webdav.seas.upenn.edu/svn/sol/vol@2489 eef5ea85-cc2e-0410-bd84-0fae1f012da8

src/ssa/ssa_dynamic.v
@@ -7,28 +7,24 @@ Require Import Arith.
 Require Import tactics.
 Require Import ssa_mem.
 Require Import monad.
+Require Import trace.
 
+(**************************************)
+(** Execution contexts *)
 Definition GenericValue := mvalue.
-Definition gptr ma := mdata_ptr ma::nil.
-
 Definition GV2nat := mvalue2nat.
+Definition GV2ptr := mvalue2mptr.
 Definition isGVUndef := isMvalueUndef.
 Definition nat2GV := nat2mvalue.
 Definition undef2GV := undef2mvalue.
+Definition ptr2GV TD p := mptr2mvalue TD p (getPointerSizeInBits TD).
 
 Definition GVMap := id -> option GenericValue.
-
-Definition updateGVMap (m:GVMap) (i:id) (v:option GenericValue) : GVMap :=
-fun i' =>
-  if (beq_nat i i')
-  then v
-  else m i'
-.
 
 Record ExecutionContext : Set := mkEC {
 CurFunction : fdef;
 CurBB       : block;
-CurInsn     : insn;
+CurInsns    : list_insn;             (* insns to run within CurBB *)
 Locals      : GVMap;                 (* LLVM values used in this invocation *)
 Args        : list GenericValue;      
 Allocas     : list mblock            (* Track memory allocated by alloca *)
@@ -45,21 +41,6 @@ Globals        : GVMap;
 Mem            : mem
 }.
 
-Definition updateLocals := updateGVMap.
-Definition updateGlobals := updateGVMap.
-
-Definition updateEnv (locals globals:GVMap) (i:id) (v:option GenericValue) : GVMap*GVMap :=
-(updateLocals locals i v,
- fun i' =>
-  if (beq_nat i i')
-  then 
-    match (locals i) with
-    | Some _ => None
-    | None => v
-    end
-  else globals i')
-.
-
 Inductive wfState : State -> Prop :=
 | wfState_intro : forall state,
   In (module_intro state.(CurTatgetData) state.(CurProducts)) state.(CurSystem) ->
@@ -71,7 +52,7 @@ Inductive wfExecutionContext : ExecutionContext -> Prop :=
   EC.(CurFunction) = fdef_intro fh lb ->
   In EC.(CurBB) lb ->
   EC.(CurBB) = block_intro l li ->
-  In EC.(CurInsn) li ->
+  (exists done, done++EC.(CurInsns)=li) ->
   wfExecutionContext EC
 .
 
@@ -88,6 +69,31 @@ Inductive wfContexts : State -> Prop :=
   wfECStack ECS ->
   wfContexts (mkState s td ps ECS g mem)
 .
+
+Definition updateGVMap (m:GVMap) (i:id) (v:option GenericValue) : GVMap :=
+fun i' =>
+  if (beq_nat i i')
+  then v
+  else m i'
+.
+
+Definition updateLocals := updateGVMap.
+Definition updateGlobals := updateGVMap.
+
+Definition updateEnv (locals globals:GVMap) (i:id) (v:option GenericValue) : GVMap*GVMap :=
+(updateLocals locals i v,
+ fun i' =>
+  if (beq_nat i i')
+  then 
+    match (locals i) with
+    | Some _ => None
+    | None => v
+    end
+  else globals i')
+.
+
+(**************************************)
+(** switchToNewBasicBlock *)
 
 Definition getCallerReturnID (Caller:insn) : option id :=
 match Caller with
@@ -147,41 +153,6 @@ match ResultValues with
 | _::ResultValues' => updateValusForNewBlock ResultValues' locals
 end.
 
-Fixpoint getEntryInsnFromInsns (li:list_insn) : option insn :=
-match li with
-| nil => None
-| (insn_phi _ _ _)::li' => getEntryInsnFromInsns li'
-| i'::li' => Some i'
-end.
-
-Definition getEntryBlock (fd:fdef) : option block :=
-match fd with
-| fdef_intro _ (b::_) => Some b
-| _ => None
-end.
-
-Definition getEntryInsn (b:block) : option insn :=
-match b with
-| block_intro _ li => getEntryInsnFromInsns li
-end.
-
-Function getNextInsnFromInsns (input:list_insn*insn) 
-         {measure (fun input'=>length (fst input'))} : option insn :=
-let (li, ci) := input in
-match li with
-| nil => None
-| i::(i'::li') => if (ci =i= i) then Some i' else (getNextInsnFromInsns (i'::li', ci))
-| _ => None
-end.
-intros.
-  simpl. auto.
-Qed.
-
-Definition getNextInsnFrom (ci:insn) (b:block) : option insn :=
-match b with
-| block_intro _ li => getNextInsnFromInsns (li,ci)
-end.
-
 (*
   SwitchToNewBasicBlock - This method is used to jump to a new basic block.
   This function handles the actual updating of block and instruction iterators
@@ -201,25 +172,21 @@ Definition switchToNewBasicBlock (Dest:block) (PrevBB:block) (locals:GVMap): (bl
   let ResultValues := getIncomingValuesForBlockFromPHINodes PNs PrevBB locals in
   (Dest, updateValusForNewBlock ResultValues locals).
 
-Fixpoint muninits (TD:layouts) (sz:nat) : mvalue :=
-match sz with
-| 0 => nil
-| S sz' => mdata_uninit::muninits TD sz'
-end.
+(**************************************)
+(** Convert const to GV with storesize, and look up GV from operands. *)
 
-(** Convert const to GV with storesize *)
 Fixpoint _const2GV (TD:layouts) (c:const) : option (GenericValue*typ) := 
 match c with
 | const_int sz n => Some (nat2GV TD sz n, typ_int sz)
-| const_undef t =>  Some (undef2GV TD t, t)
-| const_null t => Some (gptr null, t)
+| const_undef t =>  do gv <- undef2GV TD t; Some (gv, t)
+| const_null t =>   Some (ptr2GV TD null, t)
 | const_arr lc => 
          fold_left 
          (fun ogvt ogvt0 =>
           match (ogvt, ogvt0) with
           | (Some (gv, t), Some (gv0,t0)) =>
              match (getTypeAllocSize TD t0) with
-             | Some sz0 => Some ((gv++gv0)++muninits TD (sz0 - length gv0), t0)
+             | Some sz0 => Some ((gv++gv0)++muninits (sz0 - length gv0), t0)
              | None => None 
              end
           | _ => None
@@ -238,18 +205,18 @@ match c with
                | left _ (* struct_al <= sub_al *) =>
                  Some (
                   (gv++
-                  (muninits TD (sub_al - length gv0))++
+                  (muninits (sub_al - length gv0))++
                   gv0++
-                  (muninits TD (sub_sz - length gv0)),
+                  (muninits (sub_sz - length gv0)),
                   t0),
                   sub_al
                  )
                | right _ (* sub_al < struct_al *) =>
                  Some (
                   (gv++
-                  (muninits TD (sub_al - length gv0))++
+                  (muninits (sub_al - length gv0))++
                   gv0++
-                  (muninits TD (sub_sz - length gv0)),
+                  (muninits (sub_sz - length gv0)),
                   t0),
                   struct_al
                  )
@@ -263,8 +230,8 @@ match c with
          | None => None
          | Some ((gv, t), al) => 
            match (length gv) with
-           | 0 => Some (muninits TD al, t)
-           | _ => Some (gv++muninits TD (al-length gv), t)
+           | 0 => Some (muninits al, t)
+           | _ => Some (gv++muninits (al-length gv), t)
            end
          end
 end.
@@ -275,8 +242,6 @@ match (_const2GV TD c) with
 | Some (gv, t) => Some gv
 end.
 
-(* FIXME: Interpreter::getOperandValue is more complicated than this definition...
-*)
 Definition getOperandValue (TD:layouts) (v:value) (locals:GVMap) (globals:GVMap) : option GenericValue := 
 match v with
 | value_id id => 
@@ -287,20 +252,38 @@ match v with
 | value_const c => (const2GV TD c)
 end.
 
+Definition getOperandInt (TD:layouts) (sz:nat) (v:value) (locals:GVMap) (globals:GVMap) : option nat := 
+match (getOperandValue TD v locals globals) with
+| Some gi => (GV2nat TD sz gi)
+| None => None
+end.
+
+Definition isOperandUndef (TD:layouts) (t:typ) (v:value) (locals:GVMap) (globals:GVMap) : Prop  := 
+match (getOperandValue TD v locals globals) with
+| Some gi => isGVUndef TD t gi
+| None => False
+end.
+
+Definition getOperandPtr (TD:layouts) (v:value) (locals:GVMap) (globals:GVMap) : option mptr := 
+match (getOperandValue TD v locals globals) with
+| Some gi => GV2ptr TD (getPointerSize TD) gi
+| None => None
+end.
+
+Definition getOperandPtrInBits (TD:layouts) (s:sz) (v:value) (locals:GVMap) (globals:GVMap) : option mptr := 
+match (getOperandValue TD v locals globals) with
+| Some gi => GV2ptr TD s gi
+| None => None
+end.
+
+(**************************************)
+(* conversion between different lists *)
+
 Fixpoint params2OpGVs (TD:layouts) (lp:list_param) (locals:GVMap) (globals:GVMap) : list (option GenericValue):=
 match lp with
 | nil => nil
 | (_, v)::lp' => getOperandValue TD v locals globals::params2OpGVs TD lp' locals globals
 end.
-
-Fixpoint _initializeFrameValues (la:list_arg) (lg:list GenericValue) (locals:GVMap) : GVMap :=
-match (la, lg) with
-| ((_, id)::la', g::lg') => updateLocals (_initializeFrameValues la' lg' locals) id (Some g)
-| _ => locals
-end.
-
-Definition initLocals (la:list_arg) (lg:list GenericValue): GVMap := 
-_initializeFrameValues la lg (fun _ => None).
 
 Fixpoint opGVs2GVs (lg:list (option GenericValue)) : list GenericValue :=
 match lg with
@@ -312,29 +295,6 @@ end.
 Definition params2GVs (TD:layouts) (lp:list_param) (locals:GVMap) (globals:GVMap) := 
   opGVs2GVs (params2OpGVs TD lp locals globals).
 
-Record Event : Set := mkEvent { }.
-
-Inductive trace : Set :=
-| trace_nil : trace
-| trace_cons : Event -> trace -> trace
-.
-
-CoInductive Trace : Set :=
-| Trace_cons : Event -> Trace -> Trace
-.
-
-Fixpoint trace_app (tr1 tr2:trace) : trace :=
-match tr1 with
-| trace_nil => tr2
-| trace_cons e tr1' => trace_cons e (trace_app tr1' tr2)
-end.
-
-Fixpoint Trace_app (tr1:trace) (tr2:Trace) : Trace :=
-match tr1 with
-| trace_nil => tr2
-| trace_cons e tr1' => Trace_cons e (Trace_app tr1' tr2)
-end.
-
 Fixpoint intValues2Nats (TD:layouts) (lv:list value) (locals:GVMap) (globals:GVMap) : option (list nat):=
 match lv with
 | nil => Some nil
@@ -342,7 +302,7 @@ match lv with
   match (getOperandValue TD v locals globals) with
   | Some GV => 
     match (GV2nat TD 32 GV) with
-    | Some n => 
+    | Some n =>
       match (intValues2Nats TD lv' locals globals) with
       | Some ns => Some (n::ns)
       | None => None
@@ -358,7 +318,7 @@ match lv with
 | nil => Some nil
 | const_int 32 n::lv' => 
   match (GV2nat TD 32 (nat2GV TD 32 n)) with
-  | Some n => 
+  | Some n =>
     match (intConsts2Nats TD lv' locals globals) with
     | Some ns => Some (n::ns)
     | None => None
@@ -368,93 +328,63 @@ match lv with
 | _ => None
 end.
 
-Fixpoint firstn_mvalue (TD:list layout) (n:nat)(l:mvalue) {struct n} : option mvalue :=
-match n with
-| 0 => Some nil
-| S n => match l with
-         | nil => Some nil
-         | (mdata_byte b)::l => 
-            do tail <- (firstn_mvalue TD n l) ; 
-               ret (mdata_byte b::tail)
-         | (mdata_ptr ma)::l => 
-           let ps := getPointerSize TD in
-           if (le_lt_dec ps n) 
-           then 
-           do tail <- (firstn_mvalue TD (n-ps) l) ; 
-              ret (mdata_ptr ma::tail)
-           else None
-         | (mdata_uninit)::l =>
-            do tail <- (firstn_mvalue TD n l) ; 
-               ret (mdata_uninit::tail)
-         end
+(**************************************)
+(* helping functions *)
+
+Fixpoint _initializeFrameValues (la:list_arg) (lg:list GenericValue) (locals:GVMap) : GVMap :=
+match (la, lg) with
+| ((_, id)::la', g::lg') => updateLocals (_initializeFrameValues la' lg' locals) id (Some g)
+| _ => locals
 end.
 
-Fixpoint skipn_mvalue (TD:list layout) (n:nat)(l:mvalue) { struct n } : option mvalue :=
-match n with
-| 0 => Some l
-| S n => match l with
-         | nil => Some nil
-         | (mdata_byte b)::l => (skipn_mvalue TD n l) 
-         | (mdata_ptr ma)::l => 
-           let ps := getPointerSize TD in
-           if (le_lt_dec ps n) 
-           then (skipn_mvalue TD (n-ps) l) 
-           else None
-         | (mdata_uninit)::l => (skipn_mvalue TD n l) 
-         end
+Definition initLocals (la:list_arg) (lg:list GenericValue): GVMap := 
+_initializeFrameValues la lg (fun _ => None).
+
+
+Fixpoint getEntryInsnsFromInsns (li:list_insn) : option (list_insn) :=
+match li with
+| nil => None
+| (insn_phi _ _ _)::li' => getEntryInsnsFromInsns li'
+| i'::li' => Some li
 end.
 
-Definition mget (TD:list layout) (GV:mvalue) (o:moffset) (t:typ) : option mvalue :=
-do s <- getTypeStoreSize TD t;
-do tail <- skipn_mvalue TD o GV;
-   firstn_mvalue TD s tail.
+Definition getEntryBlock (fd:fdef) : option block :=
+match fd with
+| fdef_intro _ (b::_) => Some b
+| _ => None
+end.
 
+Definition getEntryInsns (b:block) : option list_insn :=
+match b with
+| block_intro _ li => getEntryInsnsFromInsns li
+end.
+
+(* FIXME : bounds check *)
 Definition extractGenericValue (TD:list layout) (locals globals:GVMap) (t:typ) (gv : GenericValue) (cidxs : list const) : option GenericValue :=
 match (intConsts2Nats TD cidxs locals globals) with
 | None => None 
 | Some idxs =>
-  match (mgetoffset TD t idxs true) with
+  match (mgetoffset TD t idxs) with
   | Some o => mget TD gv o t
   | None => None
   end
 end.
-
-Definition mset (TD:list layout) (GV:mvalue) (o:moffset) (t0:typ) (GV0:mvalue) : option mvalue :=
-do s <- getTypeStoreSize TD t0;
-do tail <- skipn_mvalue TD o GV;
-do front <- firstn_mvalue TD s tail;
-   If (beq_nat s (length GV0))
-   then ret (front++GV0++tail)
-   else None
-   endif.
 
 Definition insertGenericValue (TD:list layout) (t:typ) (gv:GenericValue) (locals globals:GVMap) 
   (cidxs:list const) (t0:typ) (gv0:GenericValue) : option GenericValue :=
 match (intConsts2Nats TD cidxs locals globals) with
 | None => None 
 | Some idxs =>
-  match (mgetoffset TD t idxs true) with
+  match (mgetoffset TD t idxs) with
   | Some o => mset TD gv o t0 gv0
   | None => None
   end
 end.
 
-Definition GEP (TD:layouts) (locals globals:GVMap) (t:typ) (ma:maddr) (vidxs:list value) (inbounds:bool) : option maddr :=
+Definition GEP (TD:layouts) (locals globals:GVMap) (t:typ) (ma:mptr) (vidxs:list value) (inbounds:bool) : option mptr :=
 match (intValues2Nats TD vidxs locals globals) with
 | None => None 
-| Some idxs => mgep TD t ma idxs inbounds
-end.
-
-Definition getOperandInt (TD:layouts) (sz:nat) (v:value) (locals:GVMap) (globals:GVMap) : option nat := 
-match (getOperandValue TD v locals globals) with
-| Some gi => GV2nat TD sz gi
-| None => None
-end.
-
-Definition isOperandUndef (TD:layouts) (sz:nat) (v:value) (locals:GVMap) (globals:GVMap) : Prop  := 
-match (getOperandValue TD v locals globals) with
-| Some gi => isGVUndef TD (typ_int sz) gi
-| None => False
+| Some idxs => mgep TD t ma idxs
 end.
 
 (***************************************************************)
@@ -463,146 +393,135 @@ end.
 Inductive dsInsn : State -> State -> trace -> Prop :=
 | dsReturn : forall S TD Ps F B RetTy Result lc gl arg id
                             F' B' I' lc' arg' EC
-                            I'' lc'' gl'' Mem Mem' als als',   
+                            Is' lc'' gl'' Mem Mem' als als',   
   Instruction.isCallInst I' = true ->
   getCallerReturnID I' = Some id ->
   (lc'', gl'') = (if (RetTy =t= typ_void) 
                   then (lc', gl) 
                   else (updateEnv lc' gl id (getOperandValue TD Result lc gl))) ->
-  getNextInsnFrom I' B' = Some I'' ->
   free_allocas Mem als = Some Mem' ->
   dsInsn 
-    (mkState S TD Ps ((mkEC F B (insn_return RetTy Result) lc arg als)::(mkEC F' B' I' lc' arg' als')::EC) gl Mem)
-    (mkState S TD Ps ((mkEC F' B' I'' lc'' arg' als')::EC) gl'' Mem')
+    (mkState S TD Ps ((mkEC F B ((insn_return RetTy Result)::nil) lc arg als)::
+                      (mkEC F' B' (I'::Is') lc' arg' als')::EC) gl Mem)
+    (mkState S TD Ps ((mkEC F' B' Is' lc'' arg' als')::EC) gl'' Mem')
     trace_nil 
 | dsBranch : forall S TD Ps F B lc gl arg Cond l1 l2 c
-                              B' I' lc' Dest EC Mem als,   
+                              B' Is' lc' Dest EC Mem als,   
   getOperandInt TD 1 Cond lc gl = Some c ->
   Some Dest = (if c
                then lookupBlockViaLabelFromSystem S l1
                else lookupBlockViaLabelFromSystem S l2) ->
   (B', lc') = (switchToNewBasicBlock Dest B lc) ->
-  getEntryInsn B' = Some I' ->
+  getEntryInsns B' = Some Is' ->
   dsInsn 
-    (mkState S TD Ps ((mkEC F B (insn_br Cond l1 l2) lc arg als)::EC) gl Mem)
-    (mkState S TD Ps ((mkEC F B' I' lc' arg als)::EC) gl Mem)
+    (mkState S TD Ps ((mkEC F B ((insn_br Cond l1 l2)::nil) lc arg als)::EC) gl Mem)
+    (mkState S TD Ps ((mkEC F B' Is' lc' arg als)::EC) gl Mem)
     trace_nil 
 | dsBranch_uncond : forall S TD Ps F B lc gl arg l
-                              B' I' lc' Dest EC Mem als,   
+                              B' Is' lc' Dest EC Mem als,   
   Some Dest = (lookupBlockViaLabelFromSystem S l) ->
   (B', lc') = (switchToNewBasicBlock Dest B lc) ->
-  getEntryInsn B = Some I' ->
+  getEntryInsns B = Some Is' ->
   dsInsn 
-    (mkState S TD Ps ((mkEC F B (insn_br_uncond l) lc arg als)::EC) gl Mem)
-    (mkState S TD Ps ((mkEC F B' I' lc' arg als)::EC) gl Mem)
+    (mkState S TD Ps ((mkEC F B ((insn_br_uncond l)::nil) lc arg als)::EC) gl Mem)
+    (mkState S TD Ps ((mkEC F B' Is' lc' arg als)::EC) gl Mem)
     trace_nil 
-| dsCall : forall S TD Ps F B lc gl arg rid fid lp
-                            B' I' EC rt la lb Mem als,
+| dsCall : forall S TD Ps F B lc gl arg rid fid lp Is
+                            B' Is' EC rt la lb Mem als,
   lookupFdefViaIDFromSystemC S fid = Some (fdef_intro (fheader_intro rt fid la) lb) ->
   getEntryBlock (fdef_intro (fheader_intro rt fid la) lb) = Some B' ->
-  getEntryInsn B' = Some I' ->
+  getEntryInsns B' = Some Is' ->
   dsInsn 
-    (mkState S TD Ps ((mkEC F B (insn_call rid rt fid lp) lc arg als)::EC) gl Mem)
+    (mkState S TD Ps ((mkEC F B ((insn_call rid rt fid lp)::Is) lc arg als)::EC) gl Mem)
     (mkState S TD Ps ((mkEC (fdef_intro (fheader_intro rt fid la) lb) 
-                                        B' I' (initLocals la (params2GVs TD lp lc gl)) 
+                                        B' Is' (initLocals la (params2GVs TD lp lc gl)) 
                                         (params2GVs TD lp lc gl) nil)::
-                                     (mkEC F B (insn_call rid rt fid lp) lc arg als)::EC) gl Mem)
+                      (mkEC F B ((insn_call rid rt fid lp)::Is) lc arg als)::EC) gl Mem)
     trace_nil 
-| dsAdd : forall S TD Ps F B lc gl lc' gl' arg id sz v1 v2 EC i1 i2 I' Mem als,
+| dsAdd : forall S TD Ps F B lc gl lc' gl' arg id sz v1 v2 EC i1 i2 Is Mem als,
   getOperandInt TD sz v1 lc gl = Some i1 ->
   getOperandInt TD sz v2 lc gl = Some i2 ->
-  getNextInsnFrom (insn_add id sz v1 v2) B = Some I' ->
   updateEnv lc gl id (Some (nat2mvalue TD sz (i1+i2))) = (lc', gl') -> 
   dsInsn 
-    (mkState S TD Ps ((mkEC F B (insn_add id sz v1 v2) lc arg als)::EC) gl Mem) 
-    (mkState S TD Ps ((mkEC F B I' lc' arg als)::EC) gl' Mem)
+    (mkState S TD Ps ((mkEC F B ((insn_add id sz v1 v2)::Is) lc arg als)::EC) gl Mem) 
+    (mkState S TD Ps ((mkEC F B Is lc' arg als)::EC) gl' Mem)
     trace_nil 
-| dsExtractValue : forall S TD Ps F B lc gl lc' gl' arg id t v gv gv' idxs EC I' Mem als,
+| dsExtractValue : forall S TD Ps F B lc gl lc' gl' arg id t v gv gv' idxs EC Is Mem als,
   getOperandValue TD v lc gl = Some gv ->
   extractGenericValue TD lc gl t gv idxs = Some gv' ->
-  getNextInsnFrom (insn_extractvalue id t v idxs) B = Some I' ->
   updateEnv lc gl id (Some gv') = (lc', gl') -> 
   dsInsn 
-    (mkState S TD Ps ((mkEC F B (insn_extractvalue id t v idxs) lc arg als)::EC) gl Mem) 
-    (mkState S TD Ps ((mkEC F B I' lc' arg als)::EC) gl' Mem)
+    (mkState S TD Ps ((mkEC F B ((insn_extractvalue id t v idxs)::Is) lc arg als)::EC) gl Mem) 
+    (mkState S TD Ps ((mkEC F B Is lc' arg als)::EC) gl' Mem)
     trace_nil 
-| dsInsertValue : forall S TD Ps F B lc gl lc' gl' arg id t v t' v' gv gv' gv'' idxs EC I' Mem als,
+| dsInsertValue : forall S TD Ps F B lc gl lc' gl' arg id t v t' v' gv gv' gv'' idxs EC Is Mem als,
   getOperandValue TD v lc gl = Some gv ->
   getOperandValue TD v' lc gl = Some gv' ->
   insertGenericValue TD t gv lc gl idxs t' gv' = Some gv'' ->
-  getNextInsnFrom (insn_insertvalue id t v t' v' idxs) B = Some I' ->
   updateEnv lc gl id (Some gv'') = (lc', gl') -> 
   dsInsn 
-    (mkState S TD Ps ((mkEC F B (insn_insertvalue id t v t' v' idxs) lc arg als)::EC) gl Mem) 
-    (mkState S TD Ps ((mkEC F B I' lc' arg als)::EC) gl' Mem)
+    (mkState S TD Ps ((mkEC F B ((insn_insertvalue id t v t' v' idxs)::Is) lc arg als)::EC) gl Mem) 
+    (mkState S TD Ps ((mkEC F B Is lc' arg als)::EC) gl' Mem)
     trace_nil 
-| dsAlloca : forall S TD Ps F B lc gl lc' gl' arg id t sz align EC I' Mem als Mem' tsz mb,
+| dsAlloca : forall S TD Ps F B lc gl lc' gl' arg id t sz align EC Is Mem als Mem' tsz mb,
   getTypeAllocSize TD t = Some tsz ->
   malloc TD Mem (tsz * sz) align = Some (Mem', mb) ->
-  getNextInsnFrom (insn_alloca id t sz align) B = Some I' ->
-  updateEnv lc gl id (Some (gptr (mb, 0))) = (lc', gl') -> 
+  updateEnv lc gl id (Some (ptr2GV TD (mb, 0))) = (lc', gl') -> 
   dsInsn 
-    (mkState S TD Ps ((mkEC F B (insn_alloca id t sz align) lc arg als)::EC) gl Mem) 
-    (mkState S TD Ps ((mkEC F B I' lc' arg (mb::als))::EC) gl' Mem')
+    (mkState S TD Ps ((mkEC F B ((insn_alloca id t sz align)::Is) lc arg als)::EC) gl Mem) 
+    (mkState S TD Ps ((mkEC F B Is lc' arg (mb::als))::EC) gl' Mem')
     trace_nil
-| dsLoad : forall S TD Ps F B lc gl lc' gl' arg id t v EC I' Mem als ma gv,
-  getOperandValue TD v lc gl = Some (gptr ma) ->
-  mload TD Mem ma t = Some gv ->
+| dsLoad : forall S TD Ps F B lc gl lc' gl' arg id t v EC Is Mem als mp gv,
+  getOperandPtr TD v lc gl = Some mp ->
+  mload TD Mem mp t = Some gv ->
   updateEnv lc gl id (Some gv) = (lc', gl') -> 
-  getNextInsnFrom (insn_load id t v) B = Some I' ->
   dsInsn 
-    (mkState S TD Ps ((mkEC F B (insn_load id t v) lc arg als)::EC) gl Mem) 
-    (mkState S TD Ps ((mkEC F B I' lc' arg als)::EC) gl' Mem)
+    (mkState S TD Ps ((mkEC F B ((insn_load id t v)::Is) lc arg als)::EC) gl Mem) 
+    (mkState S TD Ps ((mkEC F B Is lc' arg als)::EC) gl' Mem)
     trace_nil
-| dsStore : forall S TD Ps F B lc gl lc' gl' arg t v1 v2 EC I' Mem als ma2 gv1 Mem',
+| dsStore : forall S TD Ps F B lc gl lc' gl' arg t v1 v2 EC Is Mem als mp2 gv1 Mem',
   getOperandValue TD v1 lc gl = Some gv1 ->
-  getOperandValue TD v2 lc gl = Some (gptr ma2) ->
-  mstore TD Mem ma2 t gv1 = Some Mem' ->
-  getNextInsnFrom (insn_store t v1 v2) B = Some I' ->
+  getOperandPtr TD v2 lc gl = Some mp2 ->
+  mstore TD Mem mp2 t gv1 = Some Mem' ->
   dsInsn 
-    (mkState S TD Ps ((mkEC F B (insn_store t v1 v2) lc arg als)::EC) gl Mem) 
-    (mkState S TD Ps ((mkEC F B I' lc' arg als)::EC) gl' Mem)
+    (mkState S TD Ps ((mkEC F B ((insn_store t v1 v2)::Is) lc arg als)::EC) gl Mem) 
+    (mkState S TD Ps ((mkEC F B Is lc' arg als)::EC) gl' Mem)
     trace_nil
-| dsGEP : forall S TD Ps F B lc gl lc' gl' arg id t v idxs EC ma ma' I' Mem als,
-  getOperandValue TD v lc gl = Some (gptr ma) ->
-  GEP TD lc gl t ma idxs false = Some ma' ->
-  getNextInsnFrom (insn_gep id t v idxs) B = Some I' ->
-  updateEnv lc gl id (Some (gptr ma')) = (lc', gl') -> 
+| dsGEP : forall S TD Ps F B lc gl lc' gl' arg id t v idxs EC mp mp' Is Mem als,
+  getOperandPtr TD v lc gl = Some mp ->
+  GEP TD lc gl t mp idxs false = Some mp' ->
+  updateEnv lc gl id (Some (ptr2GV TD mp')) = (lc', gl') -> 
   dsInsn 
-    (mkState S TD Ps ((mkEC F B (insn_gep id t v idxs) lc arg als)::EC) gl Mem) 
-    (mkState S TD Ps ((mkEC F B I' lc' arg als)::EC) gl' Mem)
+    (mkState S TD Ps ((mkEC F B ((insn_gep id t v idxs)::Is) lc arg als)::EC) gl Mem) 
+    (mkState S TD Ps ((mkEC F B Is lc' arg als)::EC) gl' Mem)
     trace_nil 
-| dsBGEP : forall S TD Ps F B lc gl lc' gl' arg id t v idxs EC ma ma' I' Mem als,
-  getOperandValue TD v lc gl = Some (gptr ma) ->
-  GEP TD lc gl t ma idxs true = Some ma' ->
-  getNextInsnFrom (insn_bgep id t v idxs) B = Some I' ->
-  updateEnv lc gl id (Some (gptr ma')) = (lc', gl') -> 
+| dsBGEP : forall S TD Ps F B lc gl lc' gl' arg id t v idxs EC mp mp' Is Mem als,
+  getOperandPtr TD v lc gl = Some mp ->
+  GEP TD lc gl t mp idxs true = Some mp' ->
+  updateEnv lc gl id (Some (ptr2GV TD mp')) = (lc', gl') -> 
   dsInsn 
-    (mkState S TD Ps ((mkEC F B (insn_bgep id t v idxs) lc arg als)::EC) gl Mem) 
-    (mkState S TD Ps ((mkEC F B I' lc' arg als)::EC) gl' Mem)
+    (mkState S TD Ps ((mkEC F B ((insn_bgep id t v idxs)::Is) lc arg als)::EC) gl Mem) 
+    (mkState S TD Ps ((mkEC F B Is lc' arg als)::EC) gl' Mem)
     trace_nil 
-| dsInttoptr : forall S TD Ps F B lc gl arg id sz1 v1 gv1 typ2 EC I' lc' gl' Mem als,
-  getOperandValue TD v1 lc gl = Some gv1 ->
-  getNextInsnFrom (insn_inttoptr id sz1 v1 typ2) B = Some I' ->
-  updateEnv lc gl id (Some (gptr (mvalue2mptr TD sz1 gv1))) = (lc', gl') -> 
+| dsInttoptr : forall S TD Ps F B lc gl arg id sz1 v1 mp1 typ2 EC Is lc' gl' Mem als,
+  getOperandPtrInBits TD sz1 v1 lc gl = Some mp1 ->
+  updateEnv lc gl id (Some (ptr2GV TD mp1)) = (lc', gl') -> 
   dsInsn 
-    (mkState S TD Ps ((mkEC F B (insn_inttoptr id sz1 v1 typ2) lc arg als)::EC) gl Mem) 
-    (mkState S TD Ps ((mkEC F B I' lc' arg als)::EC) gl' Mem)
+    (mkState S TD Ps ((mkEC F B ((insn_inttoptr id sz1 v1 typ2)::Is) lc arg als)::EC) gl Mem) 
+    (mkState S TD Ps ((mkEC F B Is lc' arg als)::EC) gl' Mem)
     trace_nil
-| dsPtrtoint : forall S TD Ps F B lc gl arg id t1 v1 ma1 sz2 EC I' lc' gl' Mem als,
-  getOperandValue TD v1 lc gl = Some (gptr ma1) ->
-  getNextInsnFrom (insn_ptrtoint id t1 v1 sz2) B = Some I' ->
-  updateEnv lc gl id (Some (mptr2mvalue TD ma1 sz2)) = (lc', gl') -> 
+| dsPtrtoint : forall S TD Ps F B lc gl arg id t1 v1 mg1 sz2 EC Is lc' gl' Mem als,
+  getOperandPtr TD v1 lc gl = Some mg1 ->
+  updateEnv lc gl id (Some (mptr2mvalue TD mg1 sz2)) = (lc', gl') -> 
   dsInsn 
-    (mkState S TD Ps ((mkEC F B (insn_ptrtoint id t1 v1 sz2) lc arg als)::EC) gl Mem) 
-    (mkState S TD Ps ((mkEC F B I' lc' arg als)::EC) gl' Mem)
+    (mkState S TD Ps ((mkEC F B ((insn_ptrtoint id t1 v1 sz2)::Is) lc arg als)::EC) gl Mem) 
+    (mkState S TD Ps ((mkEC F B Is lc' arg als)::EC) gl' Mem)
     trace_nil
-| dsBitcast : forall S TD Ps F B lc gl arg id t1 v1 t2 EC I' lc' gl' Mem als,
-  getNextInsnFrom (insn_bitcast id t1 v1 t2) B = Some I' ->
+| dsBitcast : forall S TD Ps F B lc gl arg id t1 v1 t2 EC Is lc' gl' Mem als,
   updateEnv lc gl id (getOperandValue TD v1 lc gl) = (lc', gl') -> 
   dsInsn 
-    (mkState S TD Ps ((mkEC F B (insn_bitcast id t1 v1 t2) lc arg als)::EC) gl Mem) 
-    (mkState S TD Ps ((mkEC F B I' lc' arg als)::EC) gl' Mem)
+    (mkState S TD Ps ((mkEC F B ((insn_bitcast id t1 v1 t2)::Is) lc arg als)::EC) gl Mem) 
+    (mkState S TD Ps ((mkEC F B Is lc' arg als)::EC) gl' Mem)
     trace_nil
 .
 
@@ -615,7 +534,7 @@ match Ps with
      match (malloc TD Mem tsz align) with
      | Some (Mem', mb) => 
        do Mem'' <- mstore TD Mem' (mb, 0) t gv;
-       ret (updateGlobals gl id (Some (gptr (mb, 0))), Mem'')
+       ret (updateGlobals gl id (Some (ptr2GV TD (mb, 0))), Mem'')
      | None => None
      end
 | (product_gvar (gvar_intro id t (value_id id') align))::Ps' =>
@@ -624,7 +543,7 @@ match Ps with
      match (malloc TD Mem tsz align) with
      | Some (Mem', mb) => 
        do Mem'' <- mstore TD Mem' (mb, 0) t gv;
-       ret (updateGlobals gl id (Some (gptr (mb, 0))), Mem'')
+       ret (updateGlobals gl id (Some (ptr2GV TD (mb, 0))), Mem'')
      | None => None
      end
 | _::Ps' => genGlobalAndInitMem TD Ps' gl Mem
@@ -643,9 +562,9 @@ match (lookupFdefViaIDFromSystemC S main) with
       match (getEntryBlock CurFunction) with
       | None => None
       | Some CurBB => 
-        match (getEntryInsn CurBB) with
+        match (getEntryInsns CurBB) with
         | None => None
-        | Some CurInst =>
+        | Some CurInsts =>
           match CurFunction with 
           | fdef_intro (fheader_intro rt _ la) _ =>
             let Values := initLocals la Args in
@@ -657,7 +576,7 @@ match (lookupFdefViaIDFromSystemC S main) with
                 ((mkEC
                   CurFunction 
                   CurBB 
-                  CurInst
+                  CurInsts
                   Values 
                   Args 
                   nil
@@ -743,146 +662,136 @@ Inductive wfStates : States -> Prop :=
 Inductive nsInsn : State*trace -> States -> Prop :=
 | nsReturn : forall S TD Ps F B RetTy Result lc gl arg id
                             F' B' I' lc' arg' EC
-                            I'' lc'' gl'' tr Mem Mem' als als',   
+                            Is' lc'' gl'' tr Mem Mem' als als',   
   Instruction.isCallInst I' = true ->
   getCallerReturnID I' = Some id ->
   (lc'', gl'') = (if (RetTy =t= typ_void) 
                   then (lc', gl) 
                   else (updateEnv lc' gl id (getOperandValue TD Result lc gl))) ->
-  getNextInsnFrom I' B' = Some I'' ->
   free_allocas Mem als = Some Mem' ->
   nsInsn 
-    (mkState S TD Ps ((mkEC F B (insn_return RetTy Result) lc arg als)::(mkEC F' B' I' lc' arg' als')::EC) gl Mem, tr)
-    ((mkState S TD Ps ((mkEC F' B' I'' lc'' arg' als')::EC) gl'' Mem', tr)::nil)
+    (mkState S TD Ps ((mkEC F B ((insn_return RetTy Result)::nil) lc arg als)::
+                      (mkEC F' B' (I'::Is') lc' arg' als')::EC) gl Mem, tr)
+    ((mkState S TD Ps ((mkEC F' B' Is' lc'' arg' als')::EC) gl'' Mem', tr)::nil)
 | nsBranch_def : forall S TD Ps F B lc gl arg Cond l1 l2 c
-                              B' I' lc' Dest EC tr Mem als,   
+                              B' Is' lc' Dest EC tr Mem als,   
   getOperandInt TD 1 Cond lc gl = Some c ->
   Some Dest = (if c 
                then lookupBlockViaLabelFromSystem S l1
                else lookupBlockViaLabelFromSystem S l2) ->
   (B', lc') = (switchToNewBasicBlock Dest B lc) ->
-  getEntryInsn B' = Some I' ->
+  getEntryInsns B' = Some Is' ->
   nsInsn 
-    (mkState S TD Ps ((mkEC F B (insn_br Cond l1 l2) lc arg als)::EC) gl Mem, tr)
-    ((mkState S TD Ps ((mkEC F B' I' lc' arg als)::EC) gl Mem, tr)::nil)
+    (mkState S TD Ps ((mkEC F B ((insn_br Cond l1 l2)::nil) lc arg als)::EC) gl Mem, tr)
+    ((mkState S TD Ps ((mkEC F B' Is' lc' arg als)::EC) gl Mem, tr)::nil)
 | nsBranch_undef : forall S TD Ps F B lc arg Cond l1 l2
-                              B1' I1' lc1' B2' I2' lc2' Dest1 Dest2 EC gl tr Mem als,   
-  isOperandUndef TD 1 Cond lc gl ->
+                              B1' Is1' lc1' B2' Is2' lc2' Dest1 Dest2 EC gl tr Mem als,   
+  isOperandUndef TD (typ_int 1) Cond lc gl ->
   Some Dest1 = lookupBlockViaLabelFromSystem S l1 ->
   Some Dest2 = lookupBlockViaLabelFromSystem S l2 ->
   (B1', lc1') = (switchToNewBasicBlock Dest1 B lc) ->
   (B2', lc2') = (switchToNewBasicBlock Dest2 B lc) ->
-  getEntryInsn B1' = Some I1' ->
-  getEntryInsn B2' = Some I2' ->
+  getEntryInsns B1' = Some Is1' ->
+  getEntryInsns B2' = Some Is2' ->
   nsInsn 
-    (mkState S TD Ps ((mkEC F B (insn_br Cond l1 l2) lc arg als)::EC) gl Mem, tr)
-    ((mkState S TD Ps ((mkEC F B1' I1' lc1' arg als)::EC) gl Mem, tr)::
-     (mkState S TD Ps ((mkEC F B2' I2' lc2' arg als)::EC) gl Mem, tr)::nil)
+    (mkState S TD Ps ((mkEC F B ((insn_br Cond l1 l2)::nil) lc arg als)::EC) gl Mem, tr)
+    ((mkState S TD Ps ((mkEC F B1' Is1' lc1' arg als)::EC) gl Mem, tr)::
+     (mkState S TD Ps ((mkEC F B2' Is2' lc2' arg als)::EC) gl Mem, tr)::nil)
 | nsBranch_uncond : forall S TD Ps F B lc gl arg l
-                              B' I' lc' Dest EC tr Mem als,   
+                              B' Is' lc' Dest EC tr Mem als,   
   Some Dest = (lookupBlockViaLabelFromSystem S l) ->
   (B', lc') = (switchToNewBasicBlock Dest B lc) ->
-  getEntryInsn B = Some I' ->
+  getEntryInsns B = Some Is' ->
   nsInsn 
-    (mkState S TD Ps ((mkEC F B (insn_br_uncond l) lc arg als)::EC) gl Mem, tr)
-    ((mkState S TD Ps ((mkEC F B' I' lc' arg als)::EC) gl Mem, tr)::nil)
-| nsCall : forall S TD Ps F B lc gl arg rid fid lp
-                            Oparg' arg' F' B' I' EC rt id la lb lc' tr Mem als,
+    (mkState S TD Ps ((mkEC F B ((insn_br_uncond l)::nil) lc arg als)::EC) gl Mem, tr)
+    ((mkState S TD Ps ((mkEC F B' Is' lc' arg als)::EC) gl Mem, tr)::nil)
+| nsCall : forall S TD Ps F B lc gl arg rid fid lp Is
+                            Oparg' arg' F' B' Is' EC rt id la lb lc' tr Mem als,
   params2OpGVs TD lp lc gl = Oparg' ->   
   opGVs2GVs Oparg' = arg' ->   
   lookupFdefViaIDFromSystemC S fid = Some F' ->
   getEntryBlock F' = Some B' ->
-  getEntryInsn B' = Some I' ->
+  getEntryInsns B' = Some Is' ->
   F' = fdef_intro (fheader_intro rt id la) lb ->
   initLocals la arg' = lc' ->
   nsInsn 
-    (mkState S TD Ps ((mkEC F B (insn_call rid rt fid lp) lc arg als)::EC) gl Mem, tr)
-    ((mkState S TD Ps ((mkEC F' B' I' lc' arg' nil)::(mkEC F B (insn_call rid rt fid lp) lc arg als)::EC) gl Mem, tr)::nil)
-| nsAdd : forall S TD Ps F B lc gl lc' gl' arg id sz v1 v2 EC i1 i2 I' tr Mem als,
+    (mkState S TD Ps ((mkEC F B ((insn_call rid rt fid lp)::Is) lc arg als)::EC) gl Mem, tr)
+    ((mkState S TD Ps ((mkEC F' B' Is' lc' arg' nil)::
+                       (mkEC F B ((insn_call rid rt fid lp)::Is) lc arg als)::EC) gl Mem, tr)::nil)
+| nsAdd : forall S TD Ps F B lc gl lc' gl' arg id sz v1 v2 EC i1 i2 Is tr Mem als,
   getOperandInt TD sz v1 lc gl = Some i1 ->
   getOperandInt TD sz v2 lc gl = Some i2 ->
-  getNextInsnFrom (insn_add id sz v1 v2) B = Some I' ->
   updateEnv lc gl id (Some (nat2mvalue TD sz (i1+i2))) = (lc', gl') -> 
   nsInsn 
-    (mkState S TD Ps ((mkEC F B (insn_add id sz v1 v2) lc arg als)::EC) gl Mem, tr) 
-    ((mkState S TD Ps ((mkEC F B I' lc' arg als)::EC) gl' Mem, tr)::nil)
-| nsExtractValue : forall S TD Ps F B lc gl lc' gl' arg id t v gv gv' idxs EC I' Mem als tr,
+    (mkState S TD Ps ((mkEC F B ((insn_add id sz v1 v2)::Is) lc arg als)::EC) gl Mem, tr) 
+    ((mkState S TD Ps ((mkEC F B Is lc' arg als)::EC) gl' Mem, tr)::nil)
+| nsExtractValue : forall S TD Ps F B lc gl lc' gl' arg id t v gv gv' idxs EC Is Mem als tr,
   getOperandValue TD v lc gl = Some gv ->
   extractGenericValue TD lc gl t gv idxs = Some gv' ->
-  getNextInsnFrom (insn_extractvalue id t v idxs) B = Some I' ->
   updateEnv lc gl id (Some gv') = (lc', gl') -> 
   nsInsn 
-    (mkState S TD Ps ((mkEC F B (insn_extractvalue id t v idxs) lc arg als)::EC) gl Mem, tr) 
-    ((mkState S TD Ps ((mkEC F B I' lc' arg als)::EC) gl' Mem, tr)::nil)
-| nsInsertValue : forall S TD Ps F B lc gl lc' gl' arg id t v t' v' gv gv' gv'' idxs EC I' Mem als tr,
+    (mkState S TD Ps ((mkEC F B ((insn_extractvalue id t v idxs)::Is) lc arg als)::EC) gl Mem, tr) 
+    ((mkState S TD Ps ((mkEC F B Is lc' arg als)::EC) gl' Mem, tr)::nil)
+| nsInsertValue : forall S TD Ps F B lc gl lc' gl' arg id t v t' v' gv gv' gv'' idxs EC Is Mem als tr,
   getOperandValue TD v lc gl = Some gv ->
   getOperandValue TD v' lc gl = Some gv' ->
   insertGenericValue TD t gv lc gl idxs t' gv' = Some gv'' ->
-  getNextInsnFrom (insn_insertvalue id t v t' v' idxs) B = Some I' ->
   updateEnv lc gl id (Some gv'') = (lc', gl') -> 
   nsInsn 
-    (mkState S TD Ps ((mkEC F B (insn_insertvalue id t v t' v' idxs) lc arg als)::EC) gl Mem, tr) 
-    ((mkState S TD Ps ((mkEC F B I' lc' arg als)::EC) gl' Mem, tr)::nil)
-| nsAlloca : forall S TD Ps F B lc gl lc' gl' arg id t sz align EC I' Mem als Mem' tsz mb tr,
+    (mkState S TD Ps ((mkEC F B ((insn_insertvalue id t v t' v' idxs)::Is) lc arg als)::EC) gl Mem, tr) 
+    ((mkState S TD Ps ((mkEC F B Is lc' arg als)::EC) gl' Mem, tr)::nil)
+| nsAlloca : forall S TD Ps F B lc gl lc' gl' arg id t sz align EC Is Mem als Mem' tsz mb tr,
   getTypeAllocSize TD t = Some tsz ->
   malloc TD Mem (tsz * sz) align = Some (Mem', mb) ->
-  getNextInsnFrom (insn_alloca id t sz align) B = Some I' ->
-  updateEnv lc gl id (Some (gptr (mb, 0))) = (lc', gl') -> 
+  updateEnv lc gl id (Some (ptr2GV TD (mb, 0))) = (lc', gl') -> 
   nsInsn 
-    (mkState S TD Ps ((mkEC F B (insn_alloca id t sz align) lc arg als)::EC) gl Mem, tr) 
-    ((mkState S TD Ps ((mkEC F B I' lc' arg (mb::als))::EC) gl' Mem', tr)::nil)
-| nsLoad : forall S TD Ps F B lc gl lc' gl' arg id t v EC I' Mem als ma gv tr,
-  getOperandValue TD v lc gl = Some (gptr ma) ->
-  mload TD Mem ma t = Some gv ->
+    (mkState S TD Ps ((mkEC F B ((insn_alloca id t sz align)::Is) lc arg als)::EC) gl Mem, tr) 
+    ((mkState S TD Ps ((mkEC F B Is lc' arg (mb::als))::EC) gl' Mem', tr)::nil)
+| nsLoad : forall S TD Ps F B lc gl lc' gl' arg id t v EC Is Mem als mp gv tr,
+  getOperandPtr TD v lc gl = Some mp ->
+  mload TD Mem mp t = Some gv ->
   updateEnv lc gl id (Some gv) = (lc', gl') -> 
-  getNextInsnFrom (insn_load id t v) B = Some I' ->
   nsInsn 
-    (mkState S TD Ps ((mkEC F B (insn_load id t v) lc arg als)::EC) gl Mem, tr) 
-    ((mkState S TD Ps ((mkEC F B I' lc' arg als)::EC) gl' Mem, tr)::nil)
-| nsStore : forall S TD Ps F B lc gl lc' gl' arg t v1 v2 EC I' Mem als ma2 gv1 Mem' tr,
+    (mkState S TD Ps ((mkEC F B ((insn_load id t v)::Is) lc arg als)::EC) gl Mem, tr) 
+    ((mkState S TD Ps ((mkEC F B Is lc' arg als)::EC) gl' Mem, tr)::nil)
+| nsStore : forall S TD Ps F B lc gl lc' gl' arg t v1 v2 EC Is Mem als mp2 gv1 Mem' tr,
   getOperandValue TD v1 lc gl = Some gv1 ->
-  getOperandValue TD v2 lc gl = Some (gptr ma2) ->
-  mstore TD Mem ma2 t gv1 = Some Mem' ->
-  getNextInsnFrom (insn_store t v1 v2) B = Some I' ->
+  getOperandPtr TD v2 lc gl = Some mp2 ->
+  mstore TD Mem mp2 t gv1 = Some Mem' ->
   nsInsn 
-    (mkState S TD Ps ((mkEC F B (insn_store t v1 v2) lc arg als)::EC) gl Mem, tr) 
-    ((mkState S TD Ps ((mkEC F B I' lc' arg als)::EC) gl' Mem, tr)::nil)
-| nsGEP : forall S TD Ps F B lc gl lc' gl' arg id t v idxs EC ma ma' I' Mem als tr,
-  getOperandValue TD v lc gl = Some (gptr ma) ->
-  GEP TD lc gl t ma idxs false = Some ma' ->
-  getNextInsnFrom (insn_gep id t v idxs) B = Some I' ->
-  updateEnv lc gl id (Some (gptr ma')) = (lc', gl') -> 
+    (mkState S TD Ps ((mkEC F B ((insn_store t v1 v2)::Is) lc arg als)::EC) gl Mem, tr) 
+    ((mkState S TD Ps ((mkEC F B Is lc' arg als)::EC) gl' Mem, tr)::nil)
+| nsGEP : forall S TD Ps F B lc gl lc' gl' arg id t v idxs EC mp mp' Is Mem als tr,
+  getOperandPtr TD v lc gl = Some mp ->
+  GEP TD lc gl t mp idxs false = Some mp' ->
+  updateEnv lc gl id (Some (ptr2GV TD mp')) = (lc', gl') -> 
   nsInsn 
-    (mkState S TD Ps ((mkEC F B (insn_gep id t v idxs) lc arg als)::EC) gl Mem, tr) 
-    ((mkState S TD Ps ((mkEC F B I' lc' arg als)::EC) gl' Mem, tr)::nil)
-| nsBGEP : forall S TD Ps F B lc gl lc' gl' arg id t v idxs EC ma ma' I' Mem als tr,
-  getOperandValue TD v lc gl = Some (gptr ma) ->
-  GEP TD lc gl t ma idxs true = Some ma' ->
-  getNextInsnFrom (insn_bgep id t v idxs) B = Some I' ->
-  updateEnv lc gl id (Some (gptr ma')) = (lc', gl') -> 
+    (mkState S TD Ps ((mkEC F B ((insn_gep id t v idxs)::Is) lc arg als)::EC) gl Mem, tr) 
+    ((mkState S TD Ps ((mkEC F B Is lc' arg als)::EC) gl' Mem, tr)::nil)
+| nsBGEP : forall S TD Ps F B lc gl lc' gl' arg id t v idxs EC mp mp' Is Mem als tr,
+  getOperandPtr TD v lc gl = Some mp ->
+  GEP TD lc gl t mp idxs true = Some mp' ->
+  updateEnv lc gl id (Some (ptr2GV TD mp')) = (lc', gl') -> 
   nsInsn 
-    (mkState S TD Ps ((mkEC F B (insn_bgep id t v idxs) lc arg als)::EC) gl Mem, tr) 
-    ((mkState S TD Ps ((mkEC F B I' lc' arg als)::EC) gl' Mem, tr)::nil)
-| nsInttoptr : forall S TD Ps F B lc gl arg id sz1 v1 gv1 typ2 EC I' lc' gl' Mem als tr,
-  getOperandValue TD v1 lc gl = Some gv1 ->
-  getNextInsnFrom (insn_inttoptr id sz1 v1 typ2) B = Some I' ->
-  updateEnv lc gl id (Some (gptr (mvalue2mptr TD sz1 gv1))) = (lc', gl') -> 
+    (mkState S TD Ps ((mkEC F B ((insn_bgep id t v idxs)::Is) lc arg als)::EC) gl Mem, tr) 
+    ((mkState S TD Ps ((mkEC F B Is lc' arg als)::EC) gl' Mem, tr)::nil)
+| nsInttoptr : forall S TD Ps F B lc gl arg id sz1 v1 mp1 typ2 EC Is lc' gl' Mem als tr,
+  getOperandPtrInBits TD sz1 v1 lc gl = Some mp1 ->
+  updateEnv lc gl id (Some (ptr2GV TD mp1)) = (lc', gl') -> 
   nsInsn 
-    (mkState S TD Ps ((mkEC F B (insn_inttoptr id sz1 v1 typ2) lc arg als)::EC) gl Mem, tr) 
-    ((mkState S TD Ps ((mkEC F B I' lc' arg als)::EC) gl' Mem, tr)::nil)
-| nsPtrtoint : forall S TD Ps F B lc gl arg id t1 v1 ma1 sz2 EC I' lc' gl' Mem als tr,
-  getOperandValue TD v1 lc gl = Some (gptr ma1) ->
-  getNextInsnFrom (insn_ptrtoint id t1 v1 sz2) B = Some I' ->
-  updateEnv lc gl id (Some (mptr2mvalue TD ma1 sz2)) = (lc', gl') -> 
+    (mkState S TD Ps ((mkEC F B ((insn_inttoptr id sz1 v1 typ2)::Is) lc arg als)::EC) gl Mem, tr) 
+    ((mkState S TD Ps ((mkEC F B Is lc' arg als)::EC) gl' Mem, tr)::nil)
+| nsPtrtoint : forall S TD Ps F B lc gl arg id t1 v1 mp1 sz2 EC Is lc' gl' Mem als tr,
+  getOperandPtr TD v1 lc gl = Some mp1 ->
+  updateEnv lc gl id (Some (mptr2mvalue TD mp1 sz2)) = (lc', gl') -> 
   nsInsn 
-    (mkState S TD Ps ((mkEC F B (insn_ptrtoint id t1 v1 sz2) lc arg als)::EC) gl Mem, tr) 
-    ((mkState S TD Ps ((mkEC F B I' lc' arg als)::EC) gl' Mem, tr)::nil)
-| nsBitcast : forall S TD Ps F B lc gl arg id t1 v1 t2 EC I' lc' gl' Mem als tr,
-  getNextInsnFrom (insn_bitcast id t1 v1 t2) B = Some I' ->
+    (mkState S TD Ps ((mkEC F B ((insn_ptrtoint id t1 v1 sz2)::Is) lc arg als)::EC) gl Mem, tr) 
+    ((mkState S TD Ps ((mkEC F B Is lc' arg als)::EC) gl' Mem, tr)::nil)
+| nsBitcast : forall S TD Ps F B lc gl arg id t1 v1 t2 EC Is lc' gl' Mem als tr,
   updateEnv lc gl id (getOperandValue TD v1 lc gl) = (lc', gl') -> 
   nsInsn 
-    (mkState S TD Ps ((mkEC F B (insn_bitcast id t1 v1 t2) lc arg als)::EC) gl Mem, tr) 
-    ((mkState S TD Ps ((mkEC F B I' lc' arg als)::EC) gl' Mem, tr)::nil)
+    (mkState S TD Ps ((mkEC F B ((insn_bitcast id t1 v1 t2)::Is) lc arg als)::EC) gl Mem, tr) 
+    ((mkState S TD Ps ((mkEC F B Is lc' arg als)::EC) gl' Mem, tr)::nil)
 .
 
 Definition ns_genInitState (S:system) (main:id) (Args:list GenericValue) : option States :=
@@ -898,9 +807,9 @@ match (lookupFdefViaIDFromSystemC S main) with
       match (getEntryBlock CurFunction) with
       | None => None
       | Some CurBB => 
-        match (getEntryInsn CurBB) with
+        match (getEntryInsns CurBB) with
         | None => None
-        | Some CurInst =>
+        | Some CurInsts =>
           match CurFunction with 
           | fdef_intro (fheader_intro rt _ la) _ =>
             let Values := initLocals la Args in
@@ -912,7 +821,7 @@ match (lookupFdefViaIDFromSystemC S main) with
                 ((mkEC
                   CurFunction 
                   CurBB 
-                  CurInst
+                  CurInsts
                   Values 
                   Args 
                   nil
@@ -1001,134 +910,122 @@ Inductive ns_goeswrong : system -> id -> list GenericValue -> States -> Prop :=
 
 Inductive dbInsn : State -> State -> trace -> Prop :=
 | dbBranch : forall S TD Ps F B lc gl arg Cond l1 l2 c
-                              B' I' lc' Dest EC Mem als,   
+                              B' Is' lc' Dest EC Mem als,   
   getOperandInt TD 1 Cond lc gl = Some c ->
   Some Dest = (if c 
                then lookupBlockViaLabelFromSystem S l1
                else lookupBlockViaLabelFromSystem S l2) ->
   (B', lc') = (switchToNewBasicBlock Dest B lc) ->
-  getEntryInsn B' = Some I' ->
+  getEntryInsns B' = Some Is' ->
   dbInsn 
-    (mkState S TD Ps ((mkEC F B (insn_br Cond l1 l2) lc arg als)::EC) gl Mem)
-    (mkState S TD Ps ((mkEC F B' I' lc' arg als)::EC) gl Mem)
+    (mkState S TD Ps ((mkEC F B ((insn_br Cond l1 l2)::nil) lc arg als)::EC) gl Mem)
+    (mkState S TD Ps ((mkEC F B' Is' lc' arg als)::EC) gl Mem)
     trace_nil 
 | dbBranch_uncond : forall S TD Ps F B lc gl arg l
-                              B' I' lc' Dest EC Mem als,   
+                              B' Is' lc' Dest EC Mem als,   
   Some Dest = (lookupBlockViaLabelFromSystem S l) ->
   (B', lc') = (switchToNewBasicBlock Dest B lc) ->
-  getEntryInsn B = Some I' ->
+  getEntryInsns B = Some Is' ->
   dbInsn 
-    (mkState S TD Ps ((mkEC F B (insn_br_uncond l) lc arg als)::EC) gl Mem)
-    (mkState S TD Ps ((mkEC F B' I' lc' arg als)::EC) gl Mem)
+    (mkState S TD Ps ((mkEC F B ((insn_br_uncond l)::nil) lc arg als)::EC) gl Mem)
+    (mkState S TD Ps ((mkEC F B' Is' lc' arg als)::EC) gl Mem)
     trace_nil 
-| dbCall : forall S TD Ps F B lc gl arg rid rt fid lp gl' gl''
-                       EC Result tr I' lc'' B' lc' oGV Mem Mem' als' als Mem'',
-  dbFdef fid rt lp S TD Ps ((mkEC F B (insn_call rid rt fid lp) lc arg als)::EC) lc gl Mem lc' gl' als' Mem' B' Result tr ->
+| dbCall : forall S TD Ps F B lc gl arg rid rt fid lp gl' gl'' Is
+                       EC Result tr lc'' B' lc' oGV Mem Mem' als' als Mem'',
+  dbFdef fid rt lp S TD Ps ((mkEC F B ((insn_call rid rt fid lp)::Is) lc arg als)::EC) lc gl Mem lc' gl' als' Mem' B' Result tr ->
   getOperandValue TD Result lc' gl' = oGV -> 
   (lc'', gl'') = (if (rt =t= typ_void) 
                   then (lc, gl') 
                   else (updateEnv lc gl' rid oGV)) ->
   free_allocas Mem' als' = Some Mem'' ->
-  getNextInsnFrom (insn_call rid rt fid lp) B = Some I' ->
   dbInsn 
-    (mkState S TD Ps ((mkEC F B (insn_call rid rt fid lp) lc arg als)::EC) gl Mem) 
-    (mkState S TD Ps ((mkEC F B I' lc'' arg als)::EC) gl'' Mem'') 
+    (mkState S TD Ps ((mkEC F B ((insn_call rid rt fid lp)::Is) lc arg als)::EC) gl Mem) 
+    (mkState S TD Ps ((mkEC F B Is lc'' arg als)::EC) gl'' Mem'') 
     tr
-| dbAdd : forall S TD Ps F B lc gl lc' gl' arg id sz v1 v2 EC i1 i2 I' Mem als,
+| dbAdd : forall S TD Ps F B lc gl lc' gl' arg id sz v1 v2 EC i1 i2 Is Mem als,
   getOperandInt TD sz v1 lc gl = Some i1 ->
   getOperandInt TD sz v2 lc gl = Some i2 ->
-  getNextInsnFrom (insn_add id sz v1 v2) B = Some I' ->
   updateEnv lc gl id (Some (nat2mvalue TD sz (i1+i2))) = (lc', gl') -> 
   dbInsn 
-    (mkState S TD Ps ((mkEC F B (insn_add id sz v1 v2) lc arg als)::EC) gl Mem) 
-    (mkState S TD Ps ((mkEC F B I' lc' arg als)::EC) gl' Mem)
+    (mkState S TD Ps ((mkEC F B ((insn_add id sz v1 v2)::Is) lc arg als)::EC) gl Mem) 
+    (mkState S TD Ps ((mkEC F B Is lc' arg als)::EC) gl' Mem)
     trace_nil 
-| dbExtractValue : forall S TD Ps F B lc gl lc' gl' arg id t v gv gv' idxs EC I' Mem als,
+| dbExtractValue : forall S TD Ps F B lc gl lc' gl' arg id t v gv gv' idxs EC Is Mem als,
   getOperandValue TD v lc gl = Some gv ->
   extractGenericValue TD lc gl t gv idxs = Some gv' ->
-  getNextInsnFrom (insn_extractvalue id t v idxs) B = Some I' ->
   updateEnv lc gl id (Some gv') = (lc', gl') -> 
   dbInsn 
-    (mkState S TD Ps ((mkEC F B (insn_extractvalue id t v idxs) lc arg als)::EC) gl Mem) 
-    (mkState S TD Ps ((mkEC F B I' lc' arg als)::EC) gl' Mem)
+    (mkState S TD Ps ((mkEC F B ((insn_extractvalue id t v idxs)::Is) lc arg als)::EC) gl Mem) 
+    (mkState S TD Ps ((mkEC F B Is lc' arg als)::EC) gl' Mem)
     trace_nil 
-| dbInsertValue : forall S TD Ps F B lc gl lc' gl' arg id t v t' v' gv gv' gv'' idxs EC I' Mem als,
+| dbInsertValue : forall S TD Ps F B lc gl lc' gl' arg id t v t' v' gv gv' gv'' idxs EC Is Mem als,
   getOperandValue TD v lc gl = Some gv ->
   getOperandValue TD v' lc gl = Some gv' ->
   insertGenericValue TD t gv lc gl idxs t' gv' = Some gv'' ->
-  getNextInsnFrom (insn_insertvalue id t v t' v' idxs) B = Some I' ->
   updateEnv lc gl id (Some gv'') = (lc', gl') -> 
   dbInsn 
-    (mkState S TD Ps ((mkEC F B (insn_insertvalue id t v t' v' idxs) lc arg als)::EC) gl Mem) 
-    (mkState S TD Ps ((mkEC F B I' lc' arg als)::EC) gl' Mem)
+    (mkState S TD Ps ((mkEC F B ((insn_insertvalue id t v t' v' idxs)::Is) lc arg als)::EC) gl Mem) 
+    (mkState S TD Ps ((mkEC F B Is lc' arg als)::EC) gl' Mem)
     trace_nil 
-| dbAlloca : forall S TD Ps F B lc gl lc' gl' arg id t sz align EC I' Mem als Mem' tsz mb,
+| dbAlloca : forall S TD Ps F B lc gl lc' gl' arg id t sz align EC Is Mem als Mem' tsz mb,
   getTypeAllocSize TD t = Some tsz ->
   malloc TD Mem (tsz * sz) align = Some (Mem', mb) ->
-  getNextInsnFrom (insn_alloca id t sz align) B = Some I' ->
-  updateEnv lc gl id (Some (gptr (mb, 0))) = (lc', gl') -> 
+  updateEnv lc gl id (Some (ptr2GV TD (mb, 0))) = (lc', gl') -> 
   dbInsn 
-    (mkState S TD Ps ((mkEC F B (insn_alloca id t sz align) lc arg als)::EC) gl Mem) 
-    (mkState S TD Ps ((mkEC F B I' lc' arg (mb::als))::EC) gl' Mem')
+    (mkState S TD Ps ((mkEC F B ((insn_alloca id t sz align)::Is) lc arg als)::EC) gl Mem) 
+    (mkState S TD Ps ((mkEC F B Is lc' arg (mb::als))::EC) gl' Mem')
     trace_nil
-| dbLoad : forall S TD Ps F B lc gl lc' gl' arg id t v EC I' Mem als ma gv,
-  getOperandValue TD v lc gl = Some (gptr ma) ->
-  mload TD Mem ma t = Some gv ->
+| dbLoad : forall S TD Ps F B lc gl lc' gl' arg id t v EC Is Mem als mp gv,
+  getOperandPtr TD v lc gl = Some mp ->
+  mload TD Mem mp t = Some gv ->
   updateEnv lc gl id (Some gv) = (lc', gl') -> 
-  getNextInsnFrom (insn_load id t v) B = Some I' ->
   dbInsn 
-    (mkState S TD Ps ((mkEC F B (insn_load id t v) lc arg als)::EC) gl Mem) 
-    (mkState S TD Ps ((mkEC F B I' lc' arg als)::EC) gl' Mem)
+    (mkState S TD Ps ((mkEC F B ((insn_load id t v)::Is) lc arg als)::EC) gl Mem) 
+    (mkState S TD Ps ((mkEC F B Is lc' arg als)::EC) gl' Mem)
     trace_nil
-| dbStore : forall S TD Ps F B lc gl lc' gl' arg t v1 v2 EC I' Mem als ma2 gv1 Mem',
+| dbStore : forall S TD Ps F B lc gl lc' gl' arg t v1 v2 EC Is Mem als mp2 gv1 Mem',
   getOperandValue TD v1 lc gl = Some gv1 ->
-  getOperandValue TD v2 lc gl = Some (gptr ma2) ->
-  mstore TD Mem ma2 t gv1 = Some Mem' ->
-  getNextInsnFrom (insn_store t v1 v2) B = Some I' ->
+  getOperandPtr TD v2 lc gl = Some mp2 ->
+  mstore TD Mem mp2 t gv1 = Some Mem' ->
   dbInsn 
-    (mkState S TD Ps ((mkEC F B (insn_store t v1 v2) lc arg als)::EC) gl Mem) 
-    (mkState S TD Ps ((mkEC F B I' lc' arg als)::EC) gl' Mem)
+    (mkState S TD Ps ((mkEC F B ((insn_store t v1 v2)::Is) lc arg als)::EC) gl Mem) 
+    (mkState S TD Ps ((mkEC F B Is lc' arg als)::EC) gl' Mem)
     trace_nil
-| dbGEP : forall S TD Ps F B lc gl lc' gl' arg id t v idxs EC ma ma' I' Mem als,
-  getOperandValue TD v lc gl = Some (gptr ma) ->
-  GEP TD lc gl t ma idxs false = Some ma' ->
-  getNextInsnFrom (insn_gep id t v idxs) B = Some I' ->
-  updateEnv lc gl id (Some (gptr ma')) = (lc', gl') -> 
+| dbGEP : forall S TD Ps F B lc gl lc' gl' arg id t v idxs EC mp mp' Is Mem als,
+  getOperandPtr TD v lc gl = Some mp ->
+  GEP TD lc gl t mp idxs false = Some mp' ->
+  updateEnv lc gl id (Some (ptr2GV TD mp')) = (lc', gl') -> 
   dbInsn 
-    (mkState S TD Ps ((mkEC F B (insn_gep id t v idxs) lc arg als)::EC) gl Mem) 
-    (mkState S TD Ps ((mkEC F B I' lc' arg als)::EC) gl' Mem)
+    (mkState S TD Ps ((mkEC F B ((insn_gep id t v idxs)::Is) lc arg als)::EC) gl Mem) 
+    (mkState S TD Ps ((mkEC F B Is lc' arg als)::EC) gl' Mem)
     trace_nil 
-| dbBGEP : forall S TD Ps F B lc gl lc' gl' arg id t v idxs EC ma ma' I' Mem als,
-  getOperandValue TD v lc gl = Some (gptr ma) ->
-  GEP TD lc gl t ma idxs true = Some ma' ->
-  getNextInsnFrom (insn_bgep id t v idxs) B = Some I' ->
-  updateEnv lc gl id (Some (gptr ma')) = (lc', gl') -> 
+| dbBGEP : forall S TD Ps F B lc gl lc' gl' arg id t v idxs EC mp mp' Is Mem als,
+  getOperandPtr TD v lc gl = Some mp ->
+  GEP TD lc gl t mp idxs true = Some mp' ->
+  updateEnv lc gl id (Some (ptr2GV TD mp')) = (lc', gl') -> 
   dbInsn 
-    (mkState S TD Ps ((mkEC F B (insn_bgep id t v idxs) lc arg als)::EC) gl Mem) 
-    (mkState S TD Ps ((mkEC F B I' lc' arg als)::EC) gl' Mem)
+    (mkState S TD Ps ((mkEC F B ((insn_bgep id t v idxs)::Is) lc arg als)::EC) gl Mem) 
+    (mkState S TD Ps ((mkEC F B Is lc' arg als)::EC) gl' Mem)
     trace_nil 
-| dbInttoptr : forall S TD Ps F B lc gl arg id sz1 v1 gv1 typ2 EC I' lc' gl' Mem als,
-  getOperandValue TD v1 lc gl = Some gv1 ->
-  getNextInsnFrom (insn_inttoptr id sz1 v1 typ2) B = Some I' ->
-  updateEnv lc gl id (Some (gptr (mvalue2mptr TD sz1 gv1))) = (lc', gl') -> 
+| dbInttoptr : forall S TD Ps F B lc gl arg id sz1 v1 mp1 typ2 EC Is lc' gl' Mem als,
+  getOperandPtrInBits TD sz1 v1 lc gl = Some mp1 ->
+  updateEnv lc gl id (Some (ptr2GV TD mp1)) = (lc', gl') -> 
   dbInsn 
-    (mkState S TD Ps ((mkEC F B (insn_inttoptr id sz1 v1 typ2) lc arg als)::EC) gl Mem) 
-    (mkState S TD Ps ((mkEC F B I' lc' arg als)::EC) gl' Mem)
+    (mkState S TD Ps ((mkEC F B ((insn_inttoptr id sz1 v1 typ2)::Is) lc arg als)::EC) gl Mem) 
+    (mkState S TD Ps ((mkEC F B Is lc' arg als)::EC) gl' Mem)
     trace_nil
-| dbPtrtoint : forall S TD Ps F B lc gl arg id t1 v1 ma1 sz2 EC I' lc' gl' Mem als,
-  getOperandValue TD v1 lc gl = Some (gptr ma1) ->
-  getNextInsnFrom (insn_ptrtoint id t1 v1 sz2) B = Some I' ->
-  updateEnv lc gl id (Some (mptr2mvalue TD ma1 sz2)) = (lc', gl') -> 
+| dbPtrtoint : forall S TD Ps F B lc gl arg id t1 v1 mp1 sz2 EC Is lc' gl' Mem als,
+  getOperandPtr TD v1 lc gl = Some mp1 ->
+  updateEnv lc gl id (Some (mptr2mvalue TD mp1 sz2)) = (lc', gl') -> 
   dbInsn 
-    (mkState S TD Ps ((mkEC F B (insn_ptrtoint id t1 v1 sz2) lc arg als)::EC) gl Mem) 
-    (mkState S TD Ps ((mkEC F B I' lc' arg als)::EC) gl' Mem)
+    (mkState S TD Ps ((mkEC F B ((insn_ptrtoint id t1 v1 sz2)::Is) lc arg als)::EC) gl Mem) 
+    (mkState S TD Ps ((mkEC F B Is lc' arg als)::EC) gl' Mem)
     trace_nil
-| dbBitcast : forall S TD Ps F B lc gl arg id t1 v1 t2 EC I' lc' gl' Mem als,
-  getNextInsnFrom (insn_bitcast id t1 v1 t2) B = Some I' ->
+| dbBitcast : forall S TD Ps F B lc gl arg id t1 v1 t2 EC Is lc' gl' Mem als,
   updateEnv lc gl id (getOperandValue TD v1 lc gl) = (lc', gl') -> 
   dbInsn 
-    (mkState S TD Ps ((mkEC F B (insn_bitcast id t1 v1 t2) lc arg als)::EC) gl Mem) 
-    (mkState S TD Ps ((mkEC F B I' lc' arg als)::EC) gl' Mem)
+    (mkState S TD Ps ((mkEC F B ((insn_bitcast id t1 v1 t2)::Is) lc arg als)::EC) gl Mem) 
+    (mkState S TD Ps ((mkEC F B Is lc' arg als)::EC) gl' Mem)
     trace_nil
 with dbop : State -> State -> trace -> Prop :=
 | dbop_nil : forall S, dbop S S trace_nil
@@ -1138,27 +1035,27 @@ with dbop : State -> State -> trace -> Prop :=
     dbop S1 S3 (trace_app t1 t2)
 with dbFdef : id -> typ -> list_param -> system -> layouts -> list product -> list ExecutionContext -> GVMap -> GVMap -> mem -> GVMap -> GVMap -> list mblock -> mem -> block -> value -> trace -> Prop :=
 | dbFdef_intro : forall S TD Ps gl fid lp lc
-                            B' I' rt la lb B'' Result lc' gl' tr ECs Mem Mem' als',
+                            B' Is' rt la lb B'' Result lc' gl' tr ECs Mem Mem' als',
   lookupFdefViaIDFromSystemC S fid = Some (fdef_intro (fheader_intro rt fid la) lb) ->
   getEntryBlock (fdef_intro (fheader_intro rt fid la) lb) = Some B' ->
-  getEntryInsn B' = Some I' ->
+  getEntryInsns B' = Some Is' ->
   dbop 
     (mkState S TD Ps ((mkEC (fdef_intro (fheader_intro rt fid la) lb) 
-                             B' I' (initLocals la (params2GVs TD lp lc gl))
+                             B' Is' (initLocals la (params2GVs TD lp lc gl))
                             (params2GVs TD lp lc gl) nil)::ECs) gl Mem)
     (mkState S TD Ps ((mkEC (fdef_intro (fheader_intro rt fid la) lb) 
-                             B'' (insn_return rt Result) lc'
+                             B'' ((insn_return rt Result)::nil) lc'
                             (params2GVs TD lp lc gl) als')::ECs) gl' Mem')
     tr ->
   dbFdef fid rt lp S TD Ps ECs lc gl Mem lc' gl' als' Mem' B'' Result tr
 .
 
 CoInductive dbInsnInf : State -> Trace -> Prop :=
-| dbCallInsnInf : forall S TD Ps F B lc gl arg rid rt fid lp
+| dbCallInsnInf : forall S TD Ps F B lc gl arg rid rt fid lp Is
                        EC tr Mem als,
-  dbFdefInf fid rt lp S TD Ps ((mkEC F B (insn_call rid rt fid lp) lc arg als)::EC) lc gl Mem tr ->
+  dbFdefInf fid rt lp S TD Ps ((mkEC F B ((insn_call rid rt fid lp)::Is) lc arg als)::EC) lc gl Mem tr ->
   dbInsnInf 
-    (mkState S TD Ps ((mkEC F B (insn_call rid rt fid lp) lc arg als)::EC) gl Mem) 
+    (mkState S TD Ps ((mkEC F B ((insn_call rid rt fid lp)::Is) lc arg als)::EC) gl Mem) 
     tr
 with dbopInf : State -> Trace -> Prop :=
 | dbopInf_insn : forall state1 t1,
@@ -1170,12 +1067,12 @@ with dbopInf : State -> Trace -> Prop :=
     dbopInf state1 (Trace_app t1 t2)
 with dbFdefInf : id -> typ -> list_param -> system -> layouts -> list product -> list ExecutionContext -> GVMap -> GVMap -> mem -> Trace -> Prop :=
 | dbFdefInf_intro : forall S TD Ps lc gl fid lp
-                           B' I' rt la lb tr ECs Mem,
+                           B' Is' rt la lb tr ECs Mem,
   lookupFdefViaIDFromSystemC S fid = Some (fdef_intro (fheader_intro rt fid la) lb) ->
   getEntryBlock (fdef_intro (fheader_intro rt fid la) lb) = Some B' ->
-  getEntryInsn B' = Some I' ->
+  getEntryInsns B' = Some Is' ->
   dbopInf 
-    (mkState S TD Ps ((mkEC (fdef_intro (fheader_intro rt fid la) lb) B' I' 
+    (mkState S TD Ps ((mkEC (fdef_intro (fheader_intro rt fid la) lb) B' Is' 
                         (initLocals la (params2GVs TD lp lc gl)) 
                         (params2GVs TD lp lc gl) nil)::ECs) gl Mem)
     tr ->
@@ -1217,12 +1114,12 @@ match lc_gl_als_Mem_block_re_trs with
 | nil => nil
 | (lc', gl', als', Mem', B'', re, tr')::lc_gl_als_Mem_block_re_trs' => 
     (mkState S TD Ps ((mkEC (fdef_intro (fheader_intro rt fid la) lb) 
-                             B'' (insn_return rt re) lc'
+                             B'' ((insn_return rt re)::nil) lc'
                             (params2GVs TD lp lc gl) als')::ECs) gl' Mem', tr')::
     (returnStatesFromOp S TD Ps ECs lp lc gl rt fid la lb lc_gl_als_Mem_block_re_trs')
 end.
 
-Fixpoint updateStatesFromReturns S TD Ps F B I' lc t arg als EC rid 
+Fixpoint updateStatesFromReturns S TD Ps F B Is lc t arg als EC rid 
   (lc_gl_als_Mem_block_re_trs : list (GVMap*GVMap*list mblock*mem*block*value*trace)): option States :=
 match lc_gl_als_Mem_block_re_trs with 
 | nil => Some nil
@@ -1233,8 +1130,8 @@ match lc_gl_als_Mem_block_re_trs with
                       else (updateEnv lc gl' rid ogv)) in
   match (free_allocas Mem' als') with
   | Some Mem'' =>
-    match (updateStatesFromReturns S TD Ps F B I' lc t arg als EC rid lc_gl_als_Mem_block_re_trs') with
-    | Some states => Some ((mkState S TD Ps ((mkEC F B I' lc'' arg als)::EC) gl'' Mem'', tr)::states)
+    match (updateStatesFromReturns S TD Ps F B Is lc t arg als EC rid lc_gl_als_Mem_block_re_trs') with
+    | Some states => Some ((mkState S TD Ps ((mkEC F B Is lc'' arg als)::EC) gl'' Mem'', tr)::states)
     | None => None
     end
   | None => None
@@ -1243,129 +1140,117 @@ end.
 
 Inductive nbInsn : State*trace -> States -> Prop :=
 | nbBranch_def : forall S TD Ps F B lc gl arg  Cond l1 l2 c
-                              B' I' lc' Dest EC tr Mem als,   
+                              B' Is' lc' Dest EC tr Mem als,   
   getOperandInt TD 1 Cond lc gl = Some c ->
   Some Dest = (if c 
                then lookupBlockViaLabelFromSystem S l1
                else lookupBlockViaLabelFromSystem S l2) ->
   (B', lc') = (switchToNewBasicBlock Dest B lc) ->
-  getEntryInsn B' = Some I' ->
+  getEntryInsns B' = Some Is' ->
   nbInsn 
-    (mkState S TD Ps ((mkEC F B (insn_br Cond l1 l2) lc arg als)::EC) gl Mem, tr)
-    ((mkState S TD Ps ((mkEC F B' I' lc' arg als)::EC) gl Mem, tr)::nil)
+    (mkState S TD Ps ((mkEC F B ((insn_br Cond l1 l2)::nil) lc arg als)::EC) gl Mem, tr)
+    ((mkState S TD Ps ((mkEC F B' Is' lc' arg als)::EC) gl Mem, tr)::nil)
 | nbBranch_undef : forall S TD Ps F B lc arg Cond l1 l2
-                              B1' I1' lc1' B2' I2' lc2' Dest1 Dest2 EC tr gl Mem als,   
-  isOperandUndef TD 1 Cond lc gl ->
+                              B1' Is1' lc1' B2' Is2' lc2' Dest1 Dest2 EC tr gl Mem als,   
+  isOperandUndef TD (typ_int 1) Cond lc gl ->
   Some Dest1 = lookupBlockViaLabelFromSystem S l1 ->
   Some Dest2 = lookupBlockViaLabelFromSystem S l2 ->
   (B1', lc1') = (switchToNewBasicBlock Dest1 B lc) ->
   (B2', lc2') = (switchToNewBasicBlock Dest2 B lc) ->
-  getEntryInsn B1' = Some I1' ->
-  getEntryInsn B2' = Some I2' ->
+  getEntryInsns B1' = Some Is1' ->
+  getEntryInsns B2' = Some Is2' ->
   nbInsn 
-    (mkState S TD Ps ((mkEC F B (insn_br Cond l1 l2) lc arg als)::EC) gl Mem, tr)
-    ((mkState S TD Ps ((mkEC F B1' I1' lc1' arg als)::EC) gl Mem, tr)::
-     (mkState S TD Ps ((mkEC F B2' I2' lc2' arg als)::EC) gl Mem, tr)::nil)
+    (mkState S TD Ps ((mkEC F B ((insn_br Cond l1 l2)::nil) lc arg als)::EC) gl Mem, tr)
+    ((mkState S TD Ps ((mkEC F B1' Is1' lc1' arg als)::EC) gl Mem, tr)::
+     (mkState S TD Ps ((mkEC F B2' Is2' lc2' arg als)::EC) gl Mem, tr)::nil)
 | nbBranch_uncond : forall S TD Ps F B lc gl arg l
-                              B' I' lc' Dest EC tr Mem als,   
+                              B' Is' lc' Dest EC tr Mem als,   
   Some Dest = (lookupBlockViaLabelFromSystem S l) ->
   (B', lc') = (switchToNewBasicBlock Dest B lc) ->
-  getEntryInsn B = Some I' ->
+  getEntryInsns B = Some Is' ->
   nbInsn 
-    (mkState S TD Ps ((mkEC F B (insn_br_uncond l) lc arg als)::EC) gl Mem, tr)
-    ((mkState S TD Ps ((mkEC F B' I' lc' arg als)::EC) gl Mem, tr)::nil)
-| nbCall : forall S TD Ps F B lc gl arg rid rt fid lp
-                            EC tr lc_gl_als_Mem_block_re_trs I' Mem als states, 
-  nbFdef fid rt lp S TD Ps ((mkEC F B (insn_call rid rt fid lp) lc arg als)::EC) lc gl Mem tr lc_gl_als_Mem_block_re_trs ->
-  getNextInsnFrom (insn_call rid rt fid lp) B = Some I' ->
-  updateStatesFromReturns S TD Ps F B I' lc rt arg als EC rid lc_gl_als_Mem_block_re_trs = Some states ->
+    (mkState S TD Ps ((mkEC F B ((insn_br_uncond l)::nil) lc arg als)::EC) gl Mem, tr)
+    ((mkState S TD Ps ((mkEC F B' Is' lc' arg als)::EC) gl Mem, tr)::nil)
+| nbCall : forall S TD Ps F B lc gl arg rid rt fid lp Is
+                            EC tr lc_gl_als_Mem_block_re_trs Mem als states, 
+  nbFdef fid rt lp S TD Ps ((mkEC F B ((insn_call rid rt fid lp)::Is) lc arg als)::EC) lc gl Mem tr lc_gl_als_Mem_block_re_trs ->
+  updateStatesFromReturns S TD Ps F B Is lc rt arg als EC rid lc_gl_als_Mem_block_re_trs = Some states ->
   nbInsn 
-    (mkState S TD Ps ((mkEC F B (insn_call rid rt fid lp) lc arg als)::EC) gl Mem, tr) states    
-| nbAdd : forall S TD Ps F B lc gl lc' gl' arg id sz v1 v2 EC i1 i2 I' tr Mem als,
+    (mkState S TD Ps ((mkEC F B ((insn_call rid rt fid lp)::Is) lc arg als)::EC) gl Mem, tr) states    
+| nbAdd : forall S TD Ps F B lc gl lc' gl' arg id sz v1 v2 EC i1 i2 Is tr Mem als,
   getOperandInt TD sz v1 lc gl = Some i1 ->
   getOperandInt TD sz v2 lc gl = Some i2 ->
-  getNextInsnFrom (insn_add id sz v1 v2) B = Some I' ->
   updateEnv lc gl id (Some (nat2mvalue TD sz (i1+i2))) = (lc', gl') -> 
   nbInsn 
-    (mkState S TD Ps ((mkEC F B (insn_add id sz v1 v2) lc arg als)::EC) gl Mem, tr) 
-    ((mkState S TD Ps ((mkEC F B I' lc' arg als)::EC) gl' Mem, tr)::nil)
-| nbExtractValue : forall S TD Ps F B lc gl lc' gl' arg id t v gv gv' idxs EC I' Mem als tr,
+    (mkState S TD Ps ((mkEC F B ((insn_add id sz v1 v2)::Is) lc arg als)::EC) gl Mem, tr) 
+    ((mkState S TD Ps ((mkEC F B Is lc' arg als)::EC) gl' Mem, tr)::nil)
+| nbExtractValue : forall S TD Ps F B lc gl lc' gl' arg id t v gv gv' idxs EC Is Mem als tr,
   getOperandValue TD v lc gl = Some gv ->
   extractGenericValue TD lc gl t gv idxs = Some gv' ->
-  getNextInsnFrom (insn_extractvalue id t v idxs) B = Some I' ->
   updateEnv lc gl id (Some gv') = (lc', gl') -> 
   nbInsn 
-    (mkState S TD Ps ((mkEC F B (insn_extractvalue id t v idxs) lc arg als)::EC) gl Mem, tr) 
-    ((mkState S TD Ps ((mkEC F B I' lc' arg als)::EC) gl' Mem, tr)::nil)
-| nbInsertValue : forall S TD Ps F B lc gl lc' gl' arg id t v t' v' gv gv' gv'' idxs EC I' Mem als tr,
+    (mkState S TD Ps ((mkEC F B ((insn_extractvalue id t v idxs)::Is) lc arg als)::EC) gl Mem, tr) 
+    ((mkState S TD Ps ((mkEC F B Is lc' arg als)::EC) gl' Mem, tr)::nil)
+| nbInsertValue : forall S TD Ps F B lc gl lc' gl' arg id t v t' v' gv gv' gv'' idxs EC Is Mem als tr,
   getOperandValue TD v lc gl = Some gv ->
   getOperandValue TD v' lc gl = Some gv' ->
   insertGenericValue TD t gv lc gl idxs t' gv' = Some gv'' ->
-  getNextInsnFrom (insn_insertvalue id t v t' v' idxs) B = Some I' ->
   updateEnv lc gl id (Some gv'') = (lc', gl') -> 
   nbInsn 
-    (mkState S TD Ps ((mkEC F B (insn_insertvalue id t v t' v' idxs) lc arg als)::EC) gl Mem, tr) 
-    ((mkState S TD Ps ((mkEC F B I' lc' arg als)::EC) gl' Mem, tr)::nil)
-| nbAlloca : forall S TD Ps F B lc gl lc' gl' arg id t sz align EC I' Mem als Mem' tsz mb tr,
+    (mkState S TD Ps ((mkEC F B ((insn_insertvalue id t v t' v' idxs)::Is) lc arg als)::EC) gl Mem, tr) 
+    ((mkState S TD Ps ((mkEC F B Is lc' arg als)::EC) gl' Mem, tr)::nil)
+| nbAlloca : forall S TD Ps F B lc gl lc' gl' arg id t sz align EC Is Mem als Mem' tsz mb tr,
   getTypeAllocSize TD t = Some tsz ->
   malloc TD Mem (tsz * sz) align = Some (Mem', mb) ->
-  getNextInsnFrom (insn_alloca id t sz align) B = Some I' ->
-  updateEnv lc gl id (Some (gptr (mb, 0))) = (lc', gl') -> 
+  updateEnv lc gl id (Some (ptr2GV TD (mb, 0))) = (lc', gl') -> 
   nbInsn 
-    (mkState S TD Ps ((mkEC F B (insn_alloca id t sz align) lc arg als)::EC) gl Mem, tr) 
-    ((mkState S TD Ps ((mkEC F B I' lc' arg (mb::als))::EC) gl' Mem', tr)::nil)
-| nbLoad : forall S TD Ps F B lc gl lc' gl' arg id t v EC I' Mem als ma gv tr,
-  getOperandValue TD v lc gl = Some (gptr ma) ->
-  mload TD Mem ma t = Some gv ->
+    (mkState S TD Ps ((mkEC F B ((insn_alloca id t sz align)::Is) lc arg als)::EC) gl Mem, tr) 
+    ((mkState S TD Ps ((mkEC F B Is lc' arg (mb::als))::EC) gl' Mem', tr)::nil)
+| nbLoad : forall S TD Ps F B lc gl lc' gl' arg id t v EC Is Mem als mp gv tr,
+  getOperandPtr TD v lc gl = Some mp ->
+  mload TD Mem mp t = Some gv ->
   updateEnv lc gl id (Some gv) = (lc', gl') -> 
-  getNextInsnFrom (insn_load id t v) B = Some I' ->
   nbInsn 
-    (mkState S TD Ps ((mkEC F B (insn_load id t v) lc arg als)::EC) gl Mem, tr) 
-    ((mkState S TD Ps ((mkEC F B I' lc' arg als)::EC) gl' Mem, tr)::nil)
-| nbStore : forall S TD Ps F B lc gl lc' gl' arg t v1 v2 EC I' Mem als ma2 gv1 Mem' tr,
+    (mkState S TD Ps ((mkEC F B ((insn_load id t v)::Is) lc arg als)::EC) gl Mem, tr) 
+    ((mkState S TD Ps ((mkEC F B Is lc' arg als)::EC) gl' Mem, tr)::nil)
+| nbStore : forall S TD Ps F B lc gl lc' gl' arg t v1 v2 EC Is Mem als mp2 gv1 Mem' tr,
   getOperandValue TD v1 lc gl = Some gv1 ->
-  getOperandValue TD v2 lc gl = Some (gptr ma2) ->
-  mstore TD Mem ma2 t gv1 = Some Mem' ->
-  getNextInsnFrom (insn_store t v1 v2) B = Some I' ->
+  getOperandPtr TD v2 lc gl = Some mp2 ->
+  mstore TD Mem mp2 t gv1 = Some Mem' ->
   nbInsn 
-    (mkState S TD Ps ((mkEC F B (insn_store t v1 v2) lc arg als)::EC) gl Mem, tr) 
-    ((mkState S TD Ps ((mkEC F B I' lc' arg als)::EC) gl' Mem, tr)::nil)
-| nbGEP : forall S TD Ps F B lc gl lc' gl' arg id t v idxs EC ma ma' I' Mem als tr,
-  getOperandValue TD v lc gl = Some (gptr ma) ->
-  GEP TD lc gl t ma idxs false = Some ma' ->
-  getNextInsnFrom (insn_gep id t v idxs) B = Some I' ->
-  updateEnv lc gl id (Some (gptr ma')) = (lc', gl') -> 
+    (mkState S TD Ps ((mkEC F B ((insn_store t v1 v2)::Is) lc arg als)::EC) gl Mem, tr) 
+    ((mkState S TD Ps ((mkEC F B Is lc' arg als)::EC) gl' Mem, tr)::nil)
+| nbGEP : forall S TD Ps F B lc gl lc' gl' arg id t v idxs EC mp mp' Is Mem als tr,
+  getOperandPtr TD v lc gl = Some mp ->
+  GEP TD lc gl t mp idxs false = Some mp' ->
+  updateEnv lc gl id (Some (ptr2GV TD mp')) = (lc', gl') -> 
   nbInsn 
-    (mkState S TD Ps ((mkEC F B (insn_gep id t v idxs) lc arg als)::EC) gl Mem, tr) 
-    ((mkState S TD Ps ((mkEC F B I' lc' arg als)::EC) gl' Mem, tr)::nil)
-| nbBGEP : forall S TD Ps F B lc gl lc' gl' arg id t v idxs EC ma ma' I' Mem als tr,
-  getOperandValue TD v lc gl = Some (gptr ma) ->
-  GEP TD lc gl t ma idxs true = Some ma' ->
-  getNextInsnFrom (insn_bgep id t v idxs) B = Some I' ->
-  updateEnv lc gl id (Some (gptr ma')) = (lc', gl') -> 
+    (mkState S TD Ps ((mkEC F B ((insn_gep id t v idxs)::Is) lc arg als)::EC) gl Mem, tr) 
+    ((mkState S TD Ps ((mkEC F B Is lc' arg als)::EC) gl' Mem, tr)::nil)
+| nbBGEP : forall S TD Ps F B lc gl lc' gl' arg id t v idxs EC mp mp' Is Mem als tr,
+  getOperandPtr TD v lc gl = Some mp ->
+  GEP TD lc gl t mp idxs true = Some mp' ->
+  updateEnv lc gl id (Some (ptr2GV TD mp')) = (lc', gl') -> 
   nbInsn 
-    (mkState S TD Ps ((mkEC F B (insn_bgep id t v idxs) lc arg als)::EC) gl Mem, tr) 
-    ((mkState S TD Ps ((mkEC F B I' lc' arg als)::EC) gl' Mem, tr)::nil)
-| nbInttoptr : forall S TD Ps F B lc gl arg id sz1 v1 gv1 typ2 EC I' lc' gl' Mem als tr,
-  getOperandValue TD v1 lc gl = Some gv1 ->
-  getNextInsnFrom (insn_inttoptr id sz1 v1 typ2) B = Some I' ->
-  updateEnv lc gl id (Some (gptr (mvalue2mptr TD sz1 gv1))) = (lc', gl') -> 
+    (mkState S TD Ps ((mkEC F B ((insn_bgep id t v idxs)::Is) lc arg als)::EC) gl Mem, tr) 
+    ((mkState S TD Ps ((mkEC F B Is lc' arg als)::EC) gl' Mem, tr)::nil)
+| nbInttoptr : forall S TD Ps F B lc gl arg id sz1 v1 mp1 typ2 EC Is lc' gl' Mem als tr,
+  getOperandPtrInBits TD sz1 v1 lc gl = Some mp1 ->
+  updateEnv lc gl id (Some (ptr2GV TD mp1)) = (lc', gl') -> 
   nbInsn 
-    (mkState S TD Ps ((mkEC F B (insn_inttoptr id sz1 v1 typ2) lc arg als)::EC) gl Mem, tr) 
-    ((mkState S TD Ps ((mkEC F B I' lc' arg als)::EC) gl' Mem, tr)::nil)
-| nbPtrtoint : forall S TD Ps F B lc gl arg id t1 v1 ma1 sz2 EC I' lc' gl' Mem als tr,
-  getOperandValue TD v1 lc gl = Some (gptr ma1) ->
-  getNextInsnFrom (insn_ptrtoint id t1 v1 sz2) B = Some I' ->
-  updateEnv lc gl id (Some (mptr2mvalue TD ma1 sz2)) = (lc', gl') -> 
+    (mkState S TD Ps ((mkEC F B ((insn_inttoptr id sz1 v1 typ2)::Is) lc arg als)::EC) gl Mem, tr) 
+    ((mkState S TD Ps ((mkEC F B Is lc' arg als)::EC) gl' Mem, tr)::nil)
+| nbPtrtoint : forall S TD Ps F B lc gl arg id t1 v1 mp1 sz2 EC Is lc' gl' Mem als tr,
+  getOperandPtr TD v1 lc gl = Some mp1 ->
+  updateEnv lc gl id (Some (mptr2mvalue TD mp1 sz2)) = (lc', gl') -> 
   nbInsn 
-    (mkState S TD Ps ((mkEC F B (insn_ptrtoint id t1 v1 sz2) lc arg als)::EC) gl Mem, tr) 
-    ((mkState S TD Ps ((mkEC F B I' lc' arg als)::EC) gl' Mem, tr)::nil)
-| nbBitcast : forall S TD Ps F B lc gl arg id t1 v1 t2 EC I' lc' gl' Mem als tr,
-  getNextInsnFrom (insn_bitcast id t1 v1 t2) B = Some I' ->
+    (mkState S TD Ps ((mkEC F B ((insn_ptrtoint id t1 v1 sz2)::Is) lc arg als)::EC) gl Mem, tr) 
+    ((mkState S TD Ps ((mkEC F B Is lc' arg als)::EC) gl' Mem, tr)::nil)
+| nbBitcast : forall S TD Ps F B lc gl arg id t1 v1 t2 EC Is lc' gl' Mem als tr,
   updateEnv lc gl id (getOperandValue TD v1 lc gl) = (lc', gl') -> 
   nbInsn 
-    (mkState S TD Ps ((mkEC F B (insn_bitcast id t1 v1 t2) lc arg als)::EC) gl Mem, tr) 
-    ((mkState S TD Ps ((mkEC F B I' lc' arg als)::EC) gl' Mem, tr)::nil)
+    (mkState S TD Ps ((mkEC F B ((insn_bitcast id t1 v1 t2)::Is) lc arg als)::EC) gl Mem, tr) 
+    ((mkState S TD Ps ((mkEC F B Is lc' arg als)::EC) gl' Mem, tr)::nil)
 with nbop_star : States -> States -> Prop :=
 | nbop_star_nil : nbop_star nil nil
 | nbop_star_refl : forall state_tr states states',
@@ -1381,13 +1266,13 @@ with nbop_star : States -> States -> Prop :=
   nbop_star states1 states3 
 with nbFdef : id -> typ -> list_param -> system -> layouts -> list product -> list ExecutionContext -> GVMap -> GVMap -> mem -> trace -> list (GVMap*GVMap*list mblock*mem*block*value*trace) -> Prop :=
 | nbFdef_intro : forall S TD Ps lc gl fid lp
-                            B' I' rt la lb tr lc_gl_als_Mem_block_re_trs ECs Mem,
+                            B' Is' rt la lb tr lc_gl_als_Mem_block_re_trs ECs Mem,
   lookupFdefViaIDFromSystemC S fid = Some (fdef_intro (fheader_intro rt fid la) lb) ->
   getEntryBlock (fdef_intro (fheader_intro rt fid la) lb) = Some B' ->
-  getEntryInsn B' = Some I' ->
+  getEntryInsns B' = Some Is' ->
   nbop_star 
     ((mkState S TD Ps ((mkEC (fdef_intro (fheader_intro rt fid la) lb) 
-                         B' I' (initLocals la (params2GVs TD lp lc gl)) 
+                         B' Is' (initLocals la (params2GVs TD lp lc gl)) 
                          (params2GVs TD lp lc gl) nil)::ECs) gl Mem, tr)::nil)
     (returnStatesFromOp S TD Ps ECs lp lc gl rt fid la lb lc_gl_als_Mem_block_re_trs) ->
   nbFdef fid rt lp S TD Ps ECs lc gl Mem tr lc_gl_als_Mem_block_re_trs
@@ -1416,12 +1301,12 @@ Inductive nbop_plus : States -> States -> Prop :=
 
 CoInductive nbInsnInf : State*trace -> list Trace -> Prop :=
 | nbCallInsnInf : forall S TD Ps F B lc gl arg rid rt fid lp
-                            EC tr trs Mem als, 
+                            EC tr trs Mem als Is, 
   nbFdefInf fid rt lp S TD Ps 
-    ((mkEC F B (insn_call rid rt fid lp) lc arg als)::EC)      
+    ((mkEC F B ((insn_call rid rt fid lp)::Is) lc arg als)::EC)      
     lc gl Mem tr trs ->
   nbInsnInf 
-    (mkState S TD Ps ((mkEC F B (insn_call rid rt fid lp) lc arg als)::EC) gl Mem, tr)
+    (mkState S TD Ps ((mkEC F B ((insn_call rid rt fid lp)::Is) lc arg als)::EC) gl Mem, tr)
     trs
 with nbopInf : States -> list Trace -> Prop :=
 | nbopInf_cons : forall state_tr states tr1 tr2,
@@ -1434,13 +1319,13 @@ with nbopInf : States -> list Trace -> Prop :=
   nbopInf states1 trs 
 with nbFdefInf : id -> typ -> list_param -> system -> layouts -> list product -> list ExecutionContext -> GVMap -> GVMap -> mem -> trace -> list Trace -> Prop :=
 | nbFdefInf_intro : forall S TD Ps lc gl fid lp
-                            B' I' ECs rt la lb tr trs' Mem,
+                            B' Is' ECs rt la lb tr trs' Mem,
   lookupFdefViaIDFromSystemC S fid = Some (fdef_intro (fheader_intro rt fid la) lb) ->
   getEntryBlock (fdef_intro (fheader_intro rt fid la) lb) = Some B' ->
-  getEntryInsn B' = Some I' ->
+  getEntryInsns B' = Some Is' ->
   nbopInf 
     ((mkState S TD Ps ((mkEC (fdef_intro (fheader_intro rt fid la) lb) 
-                          B' I' (initLocals la (params2GVs TD lp lc gl)) 
+                          B' Is' (initLocals la (params2GVs TD lp lc gl)) 
                           (params2GVs TD lp lc gl) nil)::ECs) gl Mem, tr)::nil) 
     trs' ->
   nbFdefInf fid rt lp S TD Ps ECs lc gl Mem tr trs'
@@ -1489,7 +1374,7 @@ Tactic Notation "db_mutind_cases" tactic(first) tactic(c) :=
   [ c "dbBranch" | c "dbBranch_uncond" | c "dbCallInsn" |
     c "dbAdd" | c "dbExtractValue" | c "dbInsertValue" |
     c "dbAlloca" | c "dbLoad" | c "dbStore" | c "dbGEP" | c "dbBGEP" |
-    c "dbPtrtoint" | c "dbInttoptr" | c "dbBitcast" |
+    c "dbInttoptr" | c "dbPtrtoint" | c "dbBitcast" |
     c "dbop_nil" | c "dbop_cons" | c "dbFdef_intro" ].
 
 Tactic Notation "dsInsn_cases" tactic(first) tactic(c) :=
@@ -1497,7 +1382,7 @@ Tactic Notation "dsInsn_cases" tactic(first) tactic(c) :=
   [ c "dsReturn" | c "dsBranch" | c "dsBranch_uncond" | c "dsCall" |
     c "dsAdd" | c "dsExtractValue" | c "dsInsertValue" |
     c "dsAlloca" | c "dsLoad" | c "dsStore" | c "dsGEP" | c "dsBGEP" |
-        c "dsPtrtoint" | c "dsInttoptr" | c "dsBitcast" ].
+        c "dsInttoptr" | c "dsPtrtoint" | c "dsBitcast" ].
 
 Tactic Notation "dsop_star_cases" tactic(first) tactic(c) :=
   first;
@@ -1508,7 +1393,7 @@ Tactic Notation "nb_mutind_cases" tactic(first) tactic(c) :=
   [ c "nbBranch_def" | c "nbBranch_undef" | c "nbBranch_uncond" | c "nbCall" |
     c "nbAdd" | c "nbExtractValue" | c "nbInsertValue" |
     c "nbAlloca" | c "nbLoad" | c "nbStore" | c "nbGEP" | c "nbBGEP" |
-    c "nbPtrtoint" | c "nbInttoptr" | c "nbBitcast" |
+    c "nbInttoptr" | c "nbPtrtoint" | c "nbBitcast" |
     c "nbop_star_nil" | c "nbop_star_refl" | c "nbop_star_cons" | 
     c "nbop_star_trans" | c "nbFdef_intro" ].
 
@@ -1517,7 +1402,7 @@ Tactic Notation "nsInsn_cases" tactic(first) tactic(c) :=
   [ c "nsReturn" | c "nsBranch_def" | c "nsBranch_undef" | 
     c "nsBranch_uncond" | c "nsCall" | c "nsAdd" | c "nsExtractValue" | c "nsInsertValue" |
     c "nsAlloca" | c "nsLoad" | c "nsStore" | c "nsGEP" | c "nsBGEP" |
-        c "nsPtrtoint" | c "nsInttoptr" | c "nsBitcast" ].
+        c "nsInttoptr" | c "nsPtrtoint" | c "nsBitcast" ].
 
 Tactic Notation "nsop_star_cases" tactic(first) tactic(c) :=
   first;
