src/ssa/opsem_conv.v
@@ -4,42 +4,11 @@ Add LoadPath "../../../theory/metatheory".
 Require Import ssa_mem.
 Require Import ssa_dynamic.
 Require Import ssa.
+Require Import trace.
 Require Import List.
 Require Import tactics.
 Require Export Coq.Program.Equality.
 Require Export CoqListFacts.
-
-(***********************************************************)
-(** trace and Trace                                        *)
-
-Lemma trace_app_nil__eq__trace : forall tr,
-  trace_app tr trace_nil = tr.
-Proof.
-  induction tr; simpl; auto.
-    rewrite IHtr. auto.
-Qed.
-
-Lemma nil_app_trace__eq__trace : forall tr,
-  trace_app trace_nil tr = tr.
-Proof. auto. Qed.
-
-Lemma trace_app_commute : forall tr1 tr2 tr3,
-  trace_app tr1 (trace_app tr2 tr3) = trace_app (trace_app tr1 tr2) tr3.
-Proof.
-  induction tr1; intros; simpl; auto.
-    rewrite IHtr1. auto.
-Qed.
-
-Lemma nil_app_Trace__eq__Trace : forall tr,
-  Trace_app trace_nil tr = tr.
-Proof. auto. Qed.
-
-Lemma Trace_app_commute : forall tr1 tr2 tr3,
-  Trace_app tr1 (Trace_app tr2 tr3) = Trace_app (trace_app tr1 tr2) tr3.
-Proof.
-  induction tr1; intros; simpl; auto.
-    rewrite IHtr1. auto.
-Qed.
 
 (***********************************************************)
 (** det small-step                                         *)
@@ -211,16 +180,16 @@ Definition dbop__implies__dsop_star_prop state state' tr (db:dbop state state' t
   dsop_star state state' tr.
 Definition dbFdef__implies__dsop_star_prop fid rt lp S TD Ps ECs lc gl Mem lc' gl' als' Mem' B'' Result tr 
            (db:dbFdef fid rt lp S TD Ps ECs lc gl Mem lc' gl' als' Mem' B'' Result tr) := 
-  forall B' I' la lb,
+  forall B' Is' la lb,
   lookupFdefViaIDFromSystemC S fid = Some (fdef_intro (fheader_intro rt fid la) lb) ->
   getEntryBlock (fdef_intro (fheader_intro rt fid la) lb) = Some B' ->
-  getEntryInsn B' = Some I' ->
+  getEntryInsns B' = Some Is' ->
   dsop_star
     (mkState S TD Ps ((mkEC (fdef_intro (fheader_intro rt fid la) lb) 
-                             B' I' (initLocals la (params2GVs TD lp lc gl))
+                             B' Is' (initLocals la (params2GVs TD lp lc gl))
                             (params2GVs TD lp lc gl) nil)::ECs) gl Mem)
     (mkState S TD Ps ((mkEC (fdef_intro (fheader_intro rt fid la) lb) 
-                             B'' (insn_return rt Result) lc'
+                             B'' ((insn_return rt Result)::nil) lc'
                             (params2GVs TD lp lc gl) als')::ECs) gl' Mem')
     tr
   .
@@ -244,20 +213,20 @@ Proof.
   Case "dbCallInsn".
     inversion d. subst.
     assert (Hlookup:=H0).
-    apply H with (B'0:=B'0)(I':=I'0) in H0; auto.
+    apply H with (B'0:=B'0)(Is':=Is') in H0; auto.
     rewrite <- nil_app_trace__eq__trace.
     apply dsop_plus_cons with 
       (state2:=mkState S TD Ps ((mkEC (fdef_intro (fheader_intro rt fid la) lb)
-                               B'0 I'0 (initLocals la (params2GVs TD lp lc gl)) 
+                               B'0 Is' (initLocals la (params2GVs TD lp lc gl)) 
                                (params2GVs TD lp lc gl) nil)::
-                        (mkEC F B (insn_call rid rt fid lp) lc arg als)::EC) 
+                        (mkEC F B ((insn_call rid rt fid lp)::Is) lc arg als)::EC) 
                         gl Mem); auto.
     rewrite <- trace_app_nil__eq__trace.
     apply dsop_star_trans with 
       (state2:=mkState S TD Ps ((mkEC (fdef_intro (fheader_intro rt fid la) lb) 
-                               B' (insn_return rt Result) lc'
+                               B' ((insn_return rt Result)::nil) lc'
                                (params2GVs TD lp lc gl) als')::
-                        (mkEC F B (insn_call rid rt fid lp) lc arg als)::EC) 
+                        (mkEC F B ((insn_call rid rt fid lp)::Is) lc arg als)::EC) 
                         gl' Mem'); auto.
       apply dsInsn__implies__dsop_star.
       eapply dsReturn; simpl; eauto.
@@ -294,22 +263,22 @@ Proof.
   destruct db__implies__ds as [_ [J _]]. eauto.
 Qed.
 
-Lemma dbFdef__implies__dsop_star : forall fid rt lp S TD Ps ECs lc gl Mem lc' gl' als' Mem' B'' Result tr B' I' la lb,
+Lemma dbFdef__implies__dsop_star : forall fid rt lp S TD Ps ECs lc gl Mem lc' gl' als' Mem' B'' Result tr B' Is' la lb,
   dbFdef fid rt lp S TD Ps ECs lc gl Mem lc' gl' als' Mem' B'' Result tr ->
   lookupFdefViaIDFromSystemC S fid = Some (fdef_intro (fheader_intro rt fid la) lb) ->
   getEntryBlock (fdef_intro (fheader_intro rt fid la) lb) = Some B' ->
-  getEntryInsn B' = Some I' ->
+  getEntryInsns B' = Some Is' ->
   dsop_star 
     (mkState S TD Ps ((mkEC (fdef_intro (fheader_intro rt fid la) lb) 
-                             B' I' (initLocals la (params2GVs TD lp lc gl))
+                             B' Is' (initLocals la (params2GVs TD lp lc gl))
                             (params2GVs TD lp lc gl) nil)::ECs) gl Mem)
     (mkState S TD Ps ((mkEC (fdef_intro (fheader_intro rt fid la) lb) 
-                             B'' (insn_return rt Result) lc'
+                             B'' ((insn_return rt Result)::nil) lc'
                             (params2GVs TD lp lc gl) als')::ECs) gl' Mem')
     tr.
 Proof.
-  intros fid rt lp S TD Ps EC lc gl Mem lc' gl' als' Mem' B'' Result tr B' I' la lb H.
-  revert fid rt lp S TD Ps EC lc gl Mem lc' gl' als' Mem' B'' Result tr H B' I' la lb.
+  intros fid rt lp S TD Ps EC lc gl Mem lc' gl' als' Mem' B'' Result tr B' Is' la lb H.
+  revert fid rt lp S TD Ps EC lc gl Mem lc' gl' als' Mem' B'' Result tr H B' Is' la lb.
   destruct db__implies__ds as [_ [_ J]]. eauto.
 Qed.
 
@@ -341,13 +310,13 @@ Qed.
 (** First,we prove that dbInsn, dbop and dbFdef imply small-step semantics,
     by nested coinduction. *)
 
-Lemma dbFdefInf__implies__dsop_diverges : forall fid rt lp S TD Ps ECs lc gl Mem tr B' I' la lb,
+Lemma dbFdefInf__implies__dsop_diverges : forall fid rt lp S TD Ps ECs lc gl Mem tr B' Is' la lb,
   dbFdefInf fid rt lp S TD Ps ECs lc gl Mem tr ->
   lookupFdefViaIDFromSystemC S fid = Some (fdef_intro (fheader_intro rt fid la) lb) ->
   getEntryBlock (fdef_intro (fheader_intro rt fid la) lb) = Some B' ->
-  getEntryInsn B' = Some I' ->
+  getEntryInsns B' = Some Is' ->
   dsop_diverges 
-    (mkState S TD Ps ((mkEC (fdef_intro (fheader_intro rt fid la) lb) B' I' 
+    (mkState S TD Ps ((mkEC (fdef_intro (fheader_intro rt fid la) lb) B' Is' 
                         (initLocals la (params2GVs TD lp lc gl)) 
                         (params2GVs TD lp lc gl) nil)::ECs) gl Mem)
     tr.
@@ -366,12 +335,12 @@ Proof.
     inversion H; subst.
     apply dsop_diverges_intro with 
       (state2:=mkState S TD Ps ((mkEC (fdef_intro (fheader_intro rt fid la) lb)
-                               B' I' (initLocals la (params2GVs TD lp lc gl)) 
+                               B' Is' (initLocals la (params2GVs TD lp lc gl)) 
                                (params2GVs TD lp lc gl) nil)::
-                        (mkEC F B (insn_call rid rt fid lp) lc arg als)::EC) 
+                        (mkEC F B ((insn_call rid rt fid lp)::Is) lc arg als)::EC) 
                         gl Mem); 
       try solve [clear CIH_dbFdefInf CIH_dbInsnInf; auto].
-      apply CIH_dbFdefInf with (B':=B')(I':=I')(la:=la)(lb:=lb) in HdbFdefInf; auto.
+      apply CIH_dbFdefInf with (B':=B')(Is':=Is')(la:=la)(lb:=lb) in HdbFdefInf; auto.
 
   assert (forall state tr, 
           dbopInf state tr -> 
@@ -410,12 +379,12 @@ Proof.
   inversion H; subst.
   apply dsop_diverges_intro with 
     (state2:=mkState S TD Ps ((mkEC (fdef_intro (fheader_intro rt fid la) lb)
-                             B' I' (initLocals la (params2GVs TD lp lc gl)) 
+                             B' Is' (initLocals la (params2GVs TD lp lc gl)) 
                              (params2GVs TD lp lc gl) nil)::
-                      (mkEC F B (insn_call rid rt fid lp) lc arg als)::EC) 
+                      (mkEC F B ((insn_call rid rt fid lp)::Is) lc arg als)::EC) 
                       gl Mem); 
     try solve [clear CIH_dbInsnInf; auto].
-    apply dbFdefInf__implies__dsop_diverges with (B':=B')(I':=I')(la:=la)(lb:=lb) in HdbFdefInf; auto.
+    apply dbFdefInf__implies__dsop_diverges with (B':=B')(Is':=Is')(la:=la)(lb:=lb) in HdbFdefInf; auto.
 Qed.
 
 Lemma dbopInf__implies__dsop_diverges : forall state tr, 
@@ -458,27 +427,28 @@ Definition nbop_star__implies__nsop_star_prop states states' (nb:nbop_star state
   nsop_star states states'.
 Definition nbFdef__implies__nsop_star_prop fid rt lp S TD Ps ECs lc gl Mem tr lc_gl_als_Mem_block_re_trs 
            (nb:nbFdef fid rt lp S TD Ps ECs lc gl Mem tr lc_gl_als_Mem_block_re_trs) := 
-  forall B' I' la lb,
+  forall B' Is' la lb,
   lookupFdefViaIDFromSystemC S fid = Some (fdef_intro (fheader_intro rt fid la) lb) ->
   getEntryBlock (fdef_intro (fheader_intro rt fid la) lb) = Some B' ->
-  getEntryInsn B' = Some I' ->
+  getEntryInsns B' = Some Is' ->
   nsop_star
     ((mkState S TD Ps ((mkEC (fdef_intro (fheader_intro rt fid la) lb) 
-                             B' I' (initLocals la (params2GVs TD lp lc gl))
+                             B' Is' (initLocals la (params2GVs TD lp lc gl))
                             (params2GVs TD lp lc gl) nil)::ECs) gl Mem, tr)::nil)
     (returnStatesFromOp S TD Ps ECs lp lc gl rt fid la lb lc_gl_als_Mem_block_re_trs)
   .
 
-Lemma returnStatesFromOp__nsop_star__updateStatesFromReturns : forall lc_gl_als_Mem_block_re_trs S TD Ps F B rid (rt:typ) (fid:id) lp (lc:GVMap) arg als EC I' lc gl rt fid la lb states,
-  getNextInsnFrom (insn_call rid rt fid lp) B = Some I' ->
-  updateStatesFromReturns S TD Ps F B I' lc rt arg als EC rid lc_gl_als_Mem_block_re_trs = Some states ->
+Lemma returnStatesFromOp__nsop_star__updateStatesFromReturns : 
+forall lc_gl_als_Mem_block_re_trs S TD Ps F B rid (rt:typ) (fid:id) lp
+       (lc:GVMap) arg als EC Is lc gl rt fid la lb states,
+  updateStatesFromReturns S TD Ps F B Is lc rt arg als EC rid lc_gl_als_Mem_block_re_trs = Some states ->
   nsop_star
-    (returnStatesFromOp S TD Ps (mkEC F B (insn_call rid rt fid lp) lc arg als::EC)
+    (returnStatesFromOp S TD Ps (mkEC F B ((insn_call rid rt fid lp)::Is) lc arg als::EC)
                         lp lc gl rt fid la lb lc_gl_als_Mem_block_re_trs)
     states.
 Proof.
   induction lc_gl_als_Mem_block_re_trs; simpl; intros.
-  inversion H0; subst; auto.
+  inversion H; subst; auto.
 
   destruct a as [p tr]. 
   destruct p as [p re]. 
@@ -490,37 +460,35 @@ Proof.
   destruct rt0_eq_void.
   Case "rt0_is_void".
     remember (free_allocas Mem' als') as Mem''.
-    destruct Mem''; simpl in H0; try solve [inversion H0; subst].
-    remember (updateStatesFromReturns S TD Ps F B I' lc0 rt0 arg als EC rid lc_gl_als_Mem_block_re_trs) as states2.
-    destruct states2; simpl in H0; inversion H0; subst.
+    destruct Mem''; simpl in H; try solve [inversion H; subst].
+    remember (updateStatesFromReturns S TD Ps F B Is lc0 rt0 arg als EC rid lc_gl_als_Mem_block_re_trs) as states2.
+    destruct states2; simpl in H; inversion H; subst.
     assert (
-      (mkState S TD Ps (mkEC F B I' lc0 arg als::EC) gl' m, tr)::s = 
-      ((mkState S TD Ps (mkEC F B I' lc0 arg als::EC) gl' m, tr)::nil) ++ s
+      (mkState S TD Ps (mkEC F B Is lc0 arg als::EC) gl' m, tr)::s = 
+      ((mkState S TD Ps (mkEC F B Is lc0 arg als::EC) gl' m, tr)::nil) ++ s
     ) as EQ. auto.
     rewrite EQ.
     apply nsop_star_cons; auto.
       rewrite app_nil_end.
       eapply nsReturn; simpl; eauto.
         rewrite <- Heqrt0_eq_void. auto.
-      apply IHlc_gl_als_Mem_block_re_trs with (I':=I'); auto.
 
   Case "rt0_isnt_void".
     remember (updateEnv lc0 gl' rid (getOperandValue TD re lc' gl')) as lc_gl.
     destruct lc_gl as [lc'' gl''].
     remember (free_allocas Mem' als') as Mem''.
-    destruct Mem''; simpl in H0; try solve [inversion H0; subst].
-    remember (updateStatesFromReturns S TD Ps F B I' lc0 rt0 arg als EC rid lc_gl_als_Mem_block_re_trs) as states2.
-    destruct states2; simpl in H0; inversion H0; subst.
+    destruct Mem''; simpl in H; try solve [inversion H; subst].
+    remember (updateStatesFromReturns S TD Ps F B Is lc0 rt0 arg als EC rid lc_gl_als_Mem_block_re_trs) as states2.
+    destruct states2; simpl in H; inversion H; subst.
     assert (
-      (mkState S TD Ps (mkEC F B I' lc'' arg als::EC) gl'' m, tr)::s = 
-      ((mkState S TD Ps (mkEC F B I' lc'' arg als::EC) gl'' m, tr)::nil) ++ s
+      (mkState S TD Ps (mkEC F B Is lc'' arg als::EC) gl'' m, tr)::s = 
+      ((mkState S TD Ps (mkEC F B Is lc'' arg als::EC) gl'' m, tr)::nil) ++ s
     ) as EQ. auto.
     rewrite EQ.
     apply nsop_star_cons; auto.
       rewrite app_nil_end.
       eapply nsReturn; simpl; eauto.
         rewrite <- Heqrt0_eq_void. auto.
-      apply IHlc_gl_als_Mem_block_re_trs with (I':=I'); auto.
 Qed.
 
 Lemma nb__implies__ns:
@@ -541,39 +509,39 @@ Proof.
   intros; subst; simpl; 
     try solve [
       intuition |
-      apply nsop_plus_trans with (states2:=(mkState S TD Ps (mkEC F B I' lc' arg als::EC) gl' Mem, tr)::nil); 
+      apply nsop_plus_trans with (states2:=(mkState S TD Ps (mkEC F B Is lc' arg als::EC) gl' Mem, tr)::nil); 
         try solve [auto | rewrite app_nil_end; eauto] |
-      apply nsop_plus_trans with (states2:=(mkState S (module_intro TD Ps) (mkEC F B I' lc' arg als::EC) gl' Mem, tr)::nil); 
+      apply nsop_plus_trans with (states2:=(mkState S (module_intro TD Ps) (mkEC F B Is lc' arg als::EC) gl' Mem, tr)::nil); 
         try solve [auto | rewrite app_nil_end; eauto]
     ].
   Case "nbBranch_def".
-    apply nsop_plus_trans with (states2:=(mkState S TD Ps (mkEC F B' I' lc' arg als::EC) gl Mem, tr)::nil); auto.
+    apply nsop_plus_trans with (states2:=(mkState S TD Ps (mkEC F B' Is' lc' arg als::EC) gl Mem, tr)::nil); auto.
       rewrite app_nil_end; eauto.
   Case "nbBranch_undef".
-    apply nsop_plus_trans with (states2:=(mkState S TD Ps (mkEC F B1' I1' lc1' arg als::EC) gl Mem, tr)::
-                                        (mkState S TD Ps (mkEC F B2' I2' lc2' arg als::EC) gl Mem, tr)::nil); auto.
+    apply nsop_plus_trans with (states2:=(mkState S TD Ps (mkEC F B1' Is1' lc1' arg als::EC) gl Mem, tr)::
+                                        (mkState S TD Ps (mkEC F B2' Is2' lc2' arg als::EC) gl Mem, tr)::nil); auto.
       rewrite app_nil_end; eauto.
   Case "nbBranch_uncond".
-    apply nsop_plus_trans with (states2:=(mkState S TD Ps (mkEC F B' I' lc' arg als::EC) gl Mem, tr)::nil); auto.
+    apply nsop_plus_trans with (states2:=(mkState S TD Ps (mkEC F B' Is' lc' arg als::EC) gl Mem, tr)::nil); auto.
       rewrite app_nil_end; eauto.
   Case "nbCall".
     inversion n. subst.
     assert (Hlookup:=H0).
-    apply H with (B':=B')(I':=I'0) in H0; auto.
+    apply H with (B':=B')(Is':=Is') in H0; auto.
     apply nsop_plus_trans with 
       (states2:=(mkState S TD Ps ((mkEC (fdef_intro (fheader_intro rt fid la) lb)
-                               B' I'0 (initLocals la (params2GVs TD lp lc gl)) 
+                               B' Is' (initLocals la (params2GVs TD lp lc gl)) 
                                (params2GVs TD lp lc gl) nil)::
-                              (mkEC F B (insn_call rid rt fid lp) lc arg als)::EC) 
+                              (mkEC F B ((insn_call rid rt fid lp)::Is) lc arg als)::EC) 
                                gl Mem, tr)::nil); auto.
       rewrite app_nil_end; eauto.
 
       apply nsop_star_trans with 
-        (states2:=returnStatesFromOp S TD Ps (mkEC F B (insn_call rid rt fid lp) lc arg als::EC)
+        (states2:=returnStatesFromOp S TD Ps (mkEC F B ((insn_call rid rt fid lp)::Is) lc arg als::EC)
                               lp lc gl rt fid la lb lc_gl_als_Mem_block_re_trs); auto.
-      apply returnStatesFromOp__nsop_star__updateStatesFromReturns with (I':=I'); auto.
+      apply returnStatesFromOp__nsop_star__updateStatesFromReturns with (Is:=Is); auto.
   Case "nbAlloca".
-    apply nsop_plus_trans with (states2:=(mkState S TD Ps (mkEC F B I' lc' arg (mb::als)::EC) gl' Mem', tr)::nil); auto.
+    apply nsop_plus_trans with (states2:=(mkState S TD Ps (mkEC F B Is lc' arg (mb::als)::EC) gl' Mem', tr)::nil); auto.
       rewrite app_nil_end; eauto.
 
   Case "nbop_star_cons".
@@ -629,20 +597,20 @@ Proof.
     apply nsop_plus_trans with (states2:=states2); auto.
 Qed.
 
-Lemma nbFdef__implies__nsop_star : forall fid rt lp S TD Ps ECs lc gl Mem tr lc_gl_als_Mem_block_re_trs B' I' la lb,
+Lemma nbFdef__implies__nsop_star : forall fid rt lp S TD Ps ECs lc gl Mem tr lc_gl_als_Mem_block_re_trs B' Is' la lb,
   nbFdef fid rt lp S TD Ps ECs lc gl Mem tr lc_gl_als_Mem_block_re_trs ->
   lookupFdefViaIDFromSystemC S fid = Some (fdef_intro (fheader_intro rt fid la) lb) ->
   getEntryBlock (fdef_intro (fheader_intro rt fid la) lb) = Some B' ->
-  getEntryInsn B' = Some I' ->
+  getEntryInsns B' = Some Is' ->
   nsop_star
     ((mkState S TD Ps ((mkEC (fdef_intro (fheader_intro rt fid la) lb) 
-                             B' I' (initLocals la (params2GVs TD lp lc gl))
+                             B' Is' (initLocals la (params2GVs TD lp lc gl))
                             (params2GVs TD lp lc gl) nil)::ECs) gl Mem, tr)::nil)
     (returnStatesFromOp S TD Ps ECs lp lc gl rt fid la lb lc_gl_als_Mem_block_re_trs)
   .
 Proof.
-  intros fid rt lp S TD Ps ECs lc gl Mem tr lc_gl_als_Mem_block_re_trs B' I' la lb H.
-  revert fid rt lp S TD Ps ECs lc gl Mem tr lc_gl_als_Mem_block_re_trs H B' I' la lb.
+  intros fid rt lp S TD Ps ECs lc gl Mem tr lc_gl_als_Mem_block_re_trs B' Is' la lb H.
+  revert fid rt lp S TD Ps ECs lc gl Mem tr lc_gl_als_Mem_block_re_trs H B' Is' la lb.
   destruct nb__implies__ns as [_ [_ J]]. eauto.
 Qed.
 
@@ -674,13 +642,13 @@ Qed.
 (** First,we prove that nbInsn, nbop and nbFdef imply small-step semantics,
     by nested coinduction. *)
 
-Lemma nbFdefInf__implies__nsop_diverges : forall fid rt lp S TD Ps ECs lc gl Mem tr B' I' la lb trs',
+Lemma nbFdefInf__implies__nsop_diverges : forall fid rt lp S TD Ps ECs lc gl Mem tr B' Is' la lb trs',
   nbFdefInf fid rt lp S TD Ps ECs lc gl Mem tr trs' ->
   lookupFdefViaIDFromSystemC S fid = Some (fdef_intro (fheader_intro rt fid la) lb) ->
   getEntryBlock (fdef_intro (fheader_intro rt fid la) lb) = Some B' ->
-  getEntryInsn B' = Some I' ->
+  getEntryInsns B' = Some Is' ->
   nsop_diverges 
-    ((mkState S TD Ps ((mkEC (fdef_intro (fheader_intro rt fid la) lb) B' I' 
+    ((mkState S TD Ps ((mkEC (fdef_intro (fheader_intro rt fid la) lb) B' Is' 
                         (initLocals la (params2GVs TD lp lc gl)) 
                         (params2GVs TD lp lc gl) nil)::ECs) gl Mem, tr)::nil) trs'.
 Proof.
@@ -697,19 +665,19 @@ Proof.
     inversion H; subst.
     apply nsop_diverges_trans with 
       (states':=(mkState S TD Ps ((mkEC (fdef_intro (fheader_intro rt fid la) lb)
-                               B' I' (initLocals la (params2GVs TD lp lc gl)) 
+                               B' Is' (initLocals la (params2GVs TD lp lc gl)) 
                                (params2GVs TD lp lc gl) nil)::
-                        (mkEC F B (insn_call rid rt fid lp) lc arg als)::EC) 
+                        (mkEC F B ((insn_call rid rt fid lp)::Is) lc arg als)::EC) 
                         gl Mem, tr)::nil).
       apply nsop_plus_trans 
         with (states2:=(mkState S TD Ps ((mkEC (fdef_intro (fheader_intro rt fid la) lb)
-                                         B' I' (initLocals la (params2GVs TD lp lc gl)) 
+                                         B' Is' (initLocals la (params2GVs TD lp lc gl)) 
                                          (params2GVs TD lp lc gl) nil)::
-                                     (mkEC F B (insn_call rid rt fid lp) lc arg als)::EC) 
+                                     (mkEC F B ((insn_call rid rt fid lp)::Is) lc arg als)::EC) 
                                      gl Mem, tr)::nil); auto.
         rewrite app_nil_end; eauto.
       
-      apply CIH_nbFdefInf with (B':=B')(I':=I')(la:=la)(lb:=lb) in HnbFdefInf; auto.
+      apply CIH_nbFdefInf with (B':=B')(Is':=Is')(la:=la)(lb:=lb) in HnbFdefInf; auto.
 
   assert (forall states trs, 
           nbopInf states trs -> 
@@ -724,7 +692,7 @@ Proof.
       apply CIH_nbopInf in H0.
       apply nsop_diverges_trans with (states':=states2); auto.
 
-  intros fid rt lp S TD Ps ECs lc gl Mem tr B' I' la lb trs 
+  intros fid rt lp S TD Ps ECs lc gl Mem tr B' Is' la lb trs 
     HnbFdefInf Hlookup HgetEntryBlock HgetEntryInsn.
   inversion HnbFdefInf; subst.
   rewrite Hlookup in H. inversion H; subst.
@@ -746,19 +714,19 @@ Proof.
   inversion H; subst.
   apply nsop_diverges_trans with 
     (states':=(mkState S TD Ps ((mkEC (fdef_intro (fheader_intro rt fid la) lb)
-                             B' I' (initLocals la (params2GVs TD lp lc gl)) 
+                             B' Is' (initLocals la (params2GVs TD lp lc gl)) 
                              (params2GVs TD lp lc gl) nil)::
-                      (mkEC F B (insn_call rid rt fid lp) lc arg als)::EC) 
+                      (mkEC F B ((insn_call rid rt fid lp)::Is) lc arg als)::EC) 
                       gl Mem, tr)::nil).
     apply nsop_plus_trans 
       with (states2:=(mkState S TD Ps ((mkEC (fdef_intro (fheader_intro rt fid la) lb)
-                                       B' I' (initLocals la (params2GVs TD lp lc gl)) 
+                                       B' Is' (initLocals la (params2GVs TD lp lc gl)) 
                                        (params2GVs TD lp lc gl) nil)::
-                                   (mkEC F B (insn_call rid rt fid lp) lc arg als)::EC) 
+                                   (mkEC F B ((insn_call rid rt fid lp)::Is) lc arg als)::EC) 
                                    gl Mem, tr)::nil); auto.
       rewrite app_nil_end; eauto.
     
-    apply nbFdefInf__implies__nsop_diverges with (B':=B')(I':=I')(la:=la)(lb:=lb) in HnbFdefInf; auto.
+    apply nbFdefInf__implies__nsop_diverges with (B':=B')(Is':=Is')(la:=la)(lb:=lb) in HnbFdefInf; auto.
 Qed.
 
 Lemma nbopInf__implies__nsop_diverges :forall states trs, 
