src/ssa/ssa_mem.v
@@ -7,28 +7,42 @@ Require Import tactics.
 Require Export Coq.Program.Equality.
 Require Export CoqListFacts.
 Require Export targetdata.
+Require Import monad.
+Require Import Arith.
+
+(** memory address *)
+Definition maddr := nat.
 
 (** Memory is separated as blocks indexed by [mblock], contents in each block
-    are indexed by [moffset]. Addresses are encoded as pairs [mblock] and [moffset].
-    We take 0 block with 0 offset as null.
+    are indexed by [moffset]. Pointers [mptr] are encoded as pairs [mblock] and [moffset].
+    [malloca] maps [mblock] to the end address of each allocated block if the block
+    is allocated, [mblock] actually equals to the beginning address of this block.
+    We assume that there is a [null] pointer.
 *)
-Definition mblock := nat.
+Definition mblock := maddr.
+Definition malloca := mblock -> option maddr.
 Definition moffset := nat.
-Definition maddr := (mblock * moffset)%type.
+Definition mptr := (mblock * moffset)%type.
+Variable null : mptr.
 
-Definition null := (0, 0) : maddr.
-Definition uninitptr := maddr.
-
-Inductive mdata : Set :=
-| mdata_byte : nat -> mdata   (* We only need 8 bits. *) 
-| mdata_uninit  : mdata  
-| mdata_ptr : maddr -> mdata
+(** Bytes stored at each [maddr] *)
+Inductive mbyte : Set :=
+| mbyte_var : nat -> mbyte   (* We only need 8 bits. *) 
+| mbyte_uninit  : mbyte  
 .
 
-Definition mvalue := list mdata.
+(** [mem] includes a mapping from [maddr] to [mbyte], and blocks 
+    information. *)
+Record mem : Set := mkMem {
+  data   : maddr -> mbyte;
+  allocas : malloca
+}.
 
-Definition mem := mblock -> option mvalue.
-Variable initmem : mem.
+(** Values used by dynamic semantics *)
+Definition mvalue := list mbyte.
+
+(** Initially, every addr maps to uninitial byte, and no blocks are allocated. *)
+Definition initmem := mkMem (fun _ => mbyte_uninit) (fun _ => None) : mem.
 
 (** allocate memory with size and alignment *)
 Variable malloc : layouts -> mem -> nat -> nat -> option (mem * mblock)%type.
@@ -45,39 +59,59 @@ match allocas with
   end
 end.
 
-Variable mload : layouts -> mem -> maddr -> typ -> option mvalue.
+Variable mload : layouts -> mem -> mptr -> typ -> option mvalue.
 
-Variable mstore : layouts -> mem -> maddr -> typ -> mvalue -> option mem.
+Variable mstore : layouts -> mem -> mptr -> typ -> mvalue -> option mem.
 
-(** translating list of bytes to nat w.r.t typ *)
+(** translating [mvalue] to value of specific typ, failed when [mvalue] is not
+    of size [sz]. *)
 Variable mvalue2nat : layouts -> sz -> mvalue -> option nat.
-Variable mvalue2mptr : layouts -> sz -> mvalue -> maddr.
-Variable mptr2mvalue : layouts -> maddr -> sz -> mvalue.
-
-(** translating nat to mvalue with StoreSize*)
-Variable nat2mvalue : layouts -> sz -> nat -> mvalue.
-
+Variable mvalue2mptr : layouts -> sz -> mvalue -> option mptr.
 (** checking if list of bytes or uninit is undef, should all elements in list be uninits? *)
 Variable isMvalueUndef : list layout -> typ -> mvalue -> Prop.
 
-(** translating undef to mvalue with StoreSize*)
-Variable undef2mvalue : list layout -> typ -> mvalue.
+(** translating value to [mvalue] with size [sz]. *)
+Variable nat2mvalue : layouts -> nat -> sz -> mvalue.
+Variable mptr2mvalue : layouts -> mptr -> sz -> mvalue.
+(** translating undef to mvalue with StoreSize, failed when typ is not storable. *)
+Variable undef2mvalue : list layout -> typ -> option mvalue.
 
-(** compute offset in typ with list of idxs, typ and its subtypes cannot be ptr, and
-    out-of-bounds is disallowed. *)
-Variable mgetoffset : layouts -> typ -> list nat -> bool -> option moffset.
+(** addition of two [mvalue]'s with size [sz], could be none if
+    overflow happens. *)
+Variable mvalue_add : layouts -> sz -> mvalue -> mvalue -> option mvalue.
 
-(** FIXME: we should also check if sz out-of-bounds. *)
-Definition mgep (TD:layouts) (t:typ) (ma:maddr) (idxs:list nat) (inbounds:bool) : option maddr :=
+(** [sz] uninitialized [mvalue]. *)
+Fixpoint muninits (sz:nat) : mvalue :=
+match sz with
+| 0 => nil
+| S sz' => mbyte_uninit::muninits sz'
+end.
+
+(** compute offset in typ with list of idxs, typ and its subtypes cannot be ptr. *)
+Variable mgetoffset : layouts -> typ -> list nat -> option moffset.
+
+Definition mgep (TD:layouts) (t:typ) (ma:mptr) (idxs:list nat) : option mptr :=
 match ma with
 | (mb, mo) => 
   match idxs with
   | nil => None
   | (idx::idxs') =>
-    match (getTypeAllocSize TD t, mgetoffset TD t idxs' inbounds) with
+    match (getTypeAllocSize TD t, mgetoffset TD t idxs') with
     | (Some sz, Some offset) => Some (mb, mo+sz*idx+offset)
     | _ => None
     end
   end
 end.
+
+Definition mget (TD:list layout) (v:mvalue) (o:moffset) (t:typ) : option mvalue :=
+do s <- getTypeStoreSize TD t;
+   ret firstn s (skipn o v).
+
+Definition mset (TD:list layout) (v:mvalue) (o:moffset) (t0:typ) (v0:mvalue) : option mvalue :=
+do s <- getTypeStoreSize TD t0;
+   If (beq_nat s (length v0))
+   then ret ((firstn s (skipn o v))++v0++(skipn o v))
+   else None
+   endif.
+
 
